pulse/src/ocaml/plugin/generated/Pulse_Checker_Abs.ml
@@ -1,4 +1,369 @@
 open Prims
+let (check_effect_annotation :
+  Pulse_Typing_Env.env ->
+    Pulse_Syntax_Base.range ->
+      Pulse_Syntax_Base.comp ->
+        Pulse_Syntax_Base.comp -> (unit, unit) FStar_Tactics_Effect.tac_repr)
+  =
+  fun uu___3 ->
+    fun uu___2 ->
+      fun uu___1 ->
+        fun uu___ ->
+          (fun g ->
+             fun r ->
+               fun c_annot ->
+                 fun c_computed ->
+                   match (c_annot, c_computed) with
+                   | (Pulse_Syntax_Base.C_Tot uu___, Pulse_Syntax_Base.C_Tot
+                      uu___1) ->
+                       Obj.magic
+                         (Obj.repr
+                            (FStar_Tactics_Effect.lift_div_tac
+                               (fun uu___2 -> ())))
+                   | (Pulse_Syntax_Base.C_ST uu___, Pulse_Syntax_Base.C_ST
+                      uu___1) ->
+                       Obj.magic
+                         (Obj.repr
+                            (FStar_Tactics_Effect.lift_div_tac
+                               (fun uu___2 -> ())))
+                   | (Pulse_Syntax_Base.C_STAtomic (i, uu___),
+                      Pulse_Syntax_Base.C_STAtomic (j, uu___1)) ->
+                       Obj.magic
+                         (Obj.repr
+                            (if Pulse_Syntax_Base.eq_tm i j
+                             then
+                               Obj.repr
+                                 (FStar_Tactics_Effect.lift_div_tac
+                                    (fun uu___2 -> ()))
+                             else
+                               Obj.repr
+                                 (FStar_Tactics_Effect.tac_bind
+                                    (FStar_Sealed.seal
+                                       (Obj.magic
+                                          (FStar_Range.mk_range
+                                             "Pulse.Checker.Abs.fst"
+                                             (Prims.of_int (23))
+                                             (Prims.of_int (16))
+                                             (Prims.of_int (25))
+                                             (Prims.of_int (39)))))
+                                    (FStar_Sealed.seal
+                                       (Obj.magic
+                                          (FStar_Range.mk_range
+                                             "Pulse.Checker.Abs.fst"
+                                             (Prims.of_int (22))
+                                             (Prims.of_int (9))
+                                             (Prims.of_int (25))
+                                             (Prims.of_int (39)))))
+                                    (Obj.magic
+                                       (FStar_Tactics_Effect.tac_bind
+                                          (FStar_Sealed.seal
+                                             (Obj.magic
+                                                (FStar_Range.mk_range
+                                                   "Pulse.Checker.Abs.fst"
+                                                   (Prims.of_int (25))
+                                                   (Prims.of_int (18))
+                                                   (Prims.of_int (25))
+                                                   (Prims.of_int (38)))))
+                                          (FStar_Sealed.seal
+                                             (Obj.magic
+                                                (FStar_Range.mk_range
+                                                   "Pulse.Checker.Abs.fst"
+                                                   (Prims.of_int (23))
+                                                   (Prims.of_int (16))
+                                                   (Prims.of_int (25))
+                                                   (Prims.of_int (39)))))
+                                          (Obj.magic
+                                             (Pulse_Syntax_Printer.term_to_string
+                                                j))
+                                          (fun uu___3 ->
+                                             (fun uu___3 ->
+                                                Obj.magic
+                                                  (FStar_Tactics_Effect.tac_bind
+                                                     (FStar_Sealed.seal
+                                                        (Obj.magic
+                                                           (FStar_Range.mk_range
+                                                              "Pulse.Checker.Abs.fst"
+                                                              (Prims.of_int (23))
+                                                              (Prims.of_int (16))
+                                                              (Prims.of_int (25))
+                                                              (Prims.of_int (39)))))
+                                                     (FStar_Sealed.seal
+                                                        (Obj.magic
+                                                           (FStar_Range.mk_range
+                                                              "Pulse.Checker.Abs.fst"
+                                                              (Prims.of_int (23))
+                                                              (Prims.of_int (16))
+                                                              (Prims.of_int (25))
+                                                              (Prims.of_int (39)))))
+                                                     (Obj.magic
+                                                        (FStar_Tactics_Effect.tac_bind
+                                                           (FStar_Sealed.seal
+                                                              (Obj.magic
+                                                                 (FStar_Range.mk_range
+                                                                    "Pulse.Checker.Abs.fst"
+                                                                    (Prims.of_int (24))
+                                                                    (Prims.of_int (18))
+                                                                    (Prims.of_int (24))
+                                                                    (Prims.of_int (38)))))
+                                                           (FStar_Sealed.seal
+                                                              (Obj.magic
+                                                                 (FStar_Range.mk_range
+                                                                    "FStar.Printf.fst"
+                                                                    (Prims.of_int (121))
+                                                                    (Prims.of_int (8))
+                                                                    (Prims.of_int (123))
+                                                                    (Prims.of_int (44)))))
+                                                           (Obj.magic
+                                                              (Pulse_Syntax_Printer.term_to_string
+                                                                 i))
+                                                           (fun uu___4 ->
+                                                              FStar_Tactics_Effect.lift_div_tac
+                                                                (fun uu___5
+                                                                   ->
+                                                                   fun x ->
+                                                                    Prims.strcat
+                                                                    (Prims.strcat
+                                                                    "Annotated effect expects only invariants in "
+                                                                    (Prims.strcat
+                                                                    uu___4
+                                                                    " to be opened; but computed effect claims that invariants "))
+                                                                    (Prims.strcat
+                                                                    x
+                                                                    " are opened")))))
+                                                     (fun uu___4 ->
+                                                        FStar_Tactics_Effect.lift_div_tac
+                                                          (fun uu___5 ->
+                                                             uu___4 uu___3))))
+                                               uu___3)))
+                                    (fun uu___3 ->
+                                       (fun uu___3 ->
+                                          Obj.magic
+                                            (Pulse_Typing_Env.fail g
+                                               (FStar_Pervasives_Native.Some
+                                                  (i.Pulse_Syntax_Base.range1))
+                                               uu___3)) uu___3))))
+                   | (Pulse_Syntax_Base.C_STGhost (i, uu___),
+                      Pulse_Syntax_Base.C_STGhost (j, uu___1)) ->
+                       Obj.magic
+                         (Obj.repr
+                            (if Pulse_Syntax_Base.eq_tm i j
+                             then
+                               Obj.repr
+                                 (FStar_Tactics_Effect.lift_div_tac
+                                    (fun uu___2 -> ()))
+                             else
+                               Obj.repr
+                                 (FStar_Tactics_Effect.tac_bind
+                                    (FStar_Sealed.seal
+                                       (Obj.magic
+                                          (FStar_Range.mk_range
+                                             "Pulse.Checker.Abs.fst"
+                                             (Prims.of_int (23))
+                                             (Prims.of_int (16))
+                                             (Prims.of_int (25))
+                                             (Prims.of_int (39)))))
+                                    (FStar_Sealed.seal
+                                       (Obj.magic
+                                          (FStar_Range.mk_range
+                                             "Pulse.Checker.Abs.fst"
+                                             (Prims.of_int (22))
+                                             (Prims.of_int (9))
+                                             (Prims.of_int (25))
+                                             (Prims.of_int (39)))))
+                                    (Obj.magic
+                                       (FStar_Tactics_Effect.tac_bind
+                                          (FStar_Sealed.seal
+                                             (Obj.magic
+                                                (FStar_Range.mk_range
+                                                   "Pulse.Checker.Abs.fst"
+                                                   (Prims.of_int (25))
+                                                   (Prims.of_int (18))
+                                                   (Prims.of_int (25))
+                                                   (Prims.of_int (38)))))
+                                          (FStar_Sealed.seal
+                                             (Obj.magic
+                                                (FStar_Range.mk_range
+                                                   "Pulse.Checker.Abs.fst"
+                                                   (Prims.of_int (23))
+                                                   (Prims.of_int (16))
+                                                   (Prims.of_int (25))
+                                                   (Prims.of_int (39)))))
+                                          (Obj.magic
+                                             (Pulse_Syntax_Printer.term_to_string
+                                                j))
+                                          (fun uu___3 ->
+                                             (fun uu___3 ->
+                                                Obj.magic
+                                                  (FStar_Tactics_Effect.tac_bind
+                                                     (FStar_Sealed.seal
+                                                        (Obj.magic
+                                                           (FStar_Range.mk_range
+                                                              "Pulse.Checker.Abs.fst"
+                                                              (Prims.of_int (23))
+                                                              (Prims.of_int (16))
+                                                              (Prims.of_int (25))
+                                                              (Prims.of_int (39)))))
+                                                     (FStar_Sealed.seal
+                                                        (Obj.magic
+                                                           (FStar_Range.mk_range
+                                                              "Pulse.Checker.Abs.fst"
+                                                              (Prims.of_int (23))
+                                                              (Prims.of_int (16))
+                                                              (Prims.of_int (25))
+                                                              (Prims.of_int (39)))))
+                                                     (Obj.magic
+                                                        (FStar_Tactics_Effect.tac_bind
+                                                           (FStar_Sealed.seal
+                                                              (Obj.magic
+                                                                 (FStar_Range.mk_range
+                                                                    "Pulse.Checker.Abs.fst"
+                                                                    (Prims.of_int (24))
+                                                                    (Prims.of_int (18))
+                                                                    (Prims.of_int (24))
+                                                                    (Prims.of_int (38)))))
+                                                           (FStar_Sealed.seal
+                                                              (Obj.magic
+                                                                 (FStar_Range.mk_range
+                                                                    "FStar.Printf.fst"
+                                                                    (Prims.of_int (121))
+                                                                    (Prims.of_int (8))
+                                                                    (Prims.of_int (123))
+                                                                    (Prims.of_int (44)))))
+                                                           (Obj.magic
+                                                              (Pulse_Syntax_Printer.term_to_string
+                                                                 i))
+                                                           (fun uu___4 ->
+                                                              FStar_Tactics_Effect.lift_div_tac
+                                                                (fun uu___5
+                                                                   ->
+                                                                   fun x ->
+                                                                    Prims.strcat
+                                                                    (Prims.strcat
+                                                                    "Annotated effect expects only invariants in "
+                                                                    (Prims.strcat
+                                                                    uu___4
+                                                                    " to be opened; but computed effect claims that invariants "))
+                                                                    (Prims.strcat
+                                                                    x
+                                                                    " are opened")))))
+                                                     (fun uu___4 ->
+                                                        FStar_Tactics_Effect.lift_div_tac
+                                                          (fun uu___5 ->
+                                                             uu___4 uu___3))))
+                                               uu___3)))
+                                    (fun uu___3 ->
+                                       (fun uu___3 ->
+                                          Obj.magic
+                                            (Pulse_Typing_Env.fail g
+                                               (FStar_Pervasives_Native.Some
+                                                  (i.Pulse_Syntax_Base.range1))
+                                               uu___3)) uu___3))))
+                   | (uu___, uu___1) ->
+                       Obj.magic
+                         (Obj.repr
+                            (FStar_Tactics_Effect.tac_bind
+                               (FStar_Sealed.seal
+                                  (Obj.magic
+                                     (FStar_Range.mk_range
+                                        "Pulse.Checker.Abs.fst"
+                                        (Prims.of_int (28))
+                                        (Prims.of_int (11))
+                                        (Prims.of_int (30))
+                                        (Prims.of_int (45)))))
+                               (FStar_Sealed.seal
+                                  (Obj.magic
+                                     (FStar_Range.mk_range
+                                        "Pulse.Checker.Abs.fst"
+                                        (Prims.of_int (27))
+                                        (Prims.of_int (4))
+                                        (Prims.of_int (30))
+                                        (Prims.of_int (45)))))
+                               (Obj.magic
+                                  (FStar_Tactics_Effect.tac_bind
+                                     (FStar_Sealed.seal
+                                        (Obj.magic
+                                           (FStar_Range.mk_range
+                                              "Pulse.Checker.Abs.fst"
+                                              (Prims.of_int (30))
+                                              (Prims.of_int (18))
+                                              (Prims.of_int (30))
+                                              (Prims.of_int (44)))))
+                                     (FStar_Sealed.seal
+                                        (Obj.magic
+                                           (FStar_Range.mk_range
+                                              "Pulse.Checker.Abs.fst"
+                                              (Prims.of_int (28))
+                                              (Prims.of_int (11))
+                                              (Prims.of_int (30))
+                                              (Prims.of_int (45)))))
+                                     (Obj.magic
+                                        (Pulse_Syntax_Printer.tag_of_comp
+                                           c_computed))
+                                     (fun uu___2 ->
+                                        (fun uu___2 ->
+                                           Obj.magic
+                                             (FStar_Tactics_Effect.tac_bind
+                                                (FStar_Sealed.seal
+                                                   (Obj.magic
+                                                      (FStar_Range.mk_range
+                                                         "Pulse.Checker.Abs.fst"
+                                                         (Prims.of_int (28))
+                                                         (Prims.of_int (11))
+                                                         (Prims.of_int (30))
+                                                         (Prims.of_int (45)))))
+                                                (FStar_Sealed.seal
+                                                   (Obj.magic
+                                                      (FStar_Range.mk_range
+                                                         "Pulse.Checker.Abs.fst"
+                                                         (Prims.of_int (28))
+                                                         (Prims.of_int (11))
+                                                         (Prims.of_int (30))
+                                                         (Prims.of_int (45)))))
+                                                (Obj.magic
+                                                   (FStar_Tactics_Effect.tac_bind
+                                                      (FStar_Sealed.seal
+                                                         (Obj.magic
+                                                            (FStar_Range.mk_range
+                                                               "Pulse.Checker.Abs.fst"
+                                                               (Prims.of_int (29))
+                                                               (Prims.of_int (18))
+                                                               (Prims.of_int (29))
+                                                               (Prims.of_int (41)))))
+                                                      (FStar_Sealed.seal
+                                                         (Obj.magic
+                                                            (FStar_Range.mk_range
+                                                               "FStar.Printf.fst"
+                                                               (Prims.of_int (121))
+                                                               (Prims.of_int (8))
+                                                               (Prims.of_int (123))
+                                                               (Prims.of_int (44)))))
+                                                      (Obj.magic
+                                                         (Pulse_Syntax_Printer.tag_of_comp
+                                                            c_annot))
+                                                      (fun uu___3 ->
+                                                         FStar_Tactics_Effect.lift_div_tac
+                                                           (fun uu___4 ->
+                                                              fun x ->
+                                                                Prims.strcat
+                                                                  (Prims.strcat
+                                                                    "Expected effect "
+                                                                    (Prims.strcat
+                                                                    uu___3
+                                                                    " but this function body has effect "))
+                                                                  (Prims.strcat
+                                                                    x "")))))
+                                                (fun uu___3 ->
+                                                   FStar_Tactics_Effect.lift_div_tac
+                                                     (fun uu___4 ->
+                                                        uu___3 uu___2))))
+                                          uu___2)))
+                               (fun uu___2 ->
+                                  (fun uu___2 ->
+                                     Obj.magic
+                                       (Pulse_Typing_Env.fail g
+                                          (FStar_Pervasives_Native.Some r)
+                                          uu___2)) uu___2)))) uu___3 uu___2
+            uu___1 uu___
 let (check_abs :
   Pulse_Typing_Env.env ->
     Pulse_Syntax_Base.st_term ->
@@ -24,13 +389,13 @@ let (check_abs :
                   (FStar_Sealed.seal
                      (Obj.magic
                         (FStar_Range.mk_range "Pulse.Checker.Abs.fst"
-                           (Prims.of_int (24)) (Prims.of_int (14))
-                           (Prims.of_int (24)) (Prims.of_int (21)))))
+                           (Prims.of_int (43)) (Prims.of_int (14))
+                           (Prims.of_int (43)) (Prims.of_int (21)))))
                   (FStar_Sealed.seal
                      (Obj.magic
                         (FStar_Range.mk_range "Pulse.Checker.Abs.fst"
-                           (Prims.of_int (25)) (Prims.of_int (2))
-                           (Prims.of_int (59)) (Prims.of_int (27)))))
+                           (Prims.of_int (44)) (Prims.of_int (2))
+                           (Prims.of_int (88)) (Prims.of_int (27)))))
                   (FStar_Tactics_Effect.lift_div_tac
                      (fun uu___1 -> t.Pulse_Syntax_Base.range2))
                   (fun uu___1 ->
@@ -42,10 +407,8 @@ let (check_abs :
                                 { Pulse_Syntax_Base.binder_ty = t1;
                                   Pulse_Syntax_Base.binder_ppname = ppname;_};
                               Pulse_Syntax_Base.q = qual;
-                              Pulse_Syntax_Base.pre1 = pre_hint;
-                              Pulse_Syntax_Base.body = body;
-                              Pulse_Syntax_Base.ret_ty = ret_ty;
-                              Pulse_Syntax_Base.post1 = post_hint_body;_}
+                              Pulse_Syntax_Base.ascription = c;
+                              Pulse_Syntax_Base.body = body;_}
                             ->
                             Obj.magic
                               (FStar_Tactics_Effect.tac_bind
@@ -53,17 +416,17 @@ let (check_abs :
                                     (Obj.magic
                                        (FStar_Range.mk_range
                                           "Pulse.Checker.Abs.fst"
-                                          (Prims.of_int (28))
+                                          (Prims.of_int (47))
                                           (Prims.of_int (24))
-                                          (Prims.of_int (28))
+                                          (Prims.of_int (47))
                                           (Prims.of_int (38)))))
                                  (FStar_Sealed.seal
                                     (Obj.magic
                                        (FStar_Range.mk_range
                                           "Pulse.Checker.Abs.fst"
-                                          (Prims.of_int (26))
-                                          (Prims.of_int (113))
-                                          (Prims.of_int (59))
+                                          (Prims.of_int (45))
+                                          (Prims.of_int (84))
+                                          (Prims.of_int (88))
                                           (Prims.of_int (27)))))
                                  (Obj.magic
                                     (Pulse_Checker_Pure.check_term g t1))
@@ -78,17 +441,17 @@ let (check_abs :
                                                    (Obj.magic
                                                       (FStar_Range.mk_range
                                                          "Pulse.Checker.Abs.fst"
-                                                         (Prims.of_int (29))
+                                                         (Prims.of_int (48))
                                                          (Prims.of_int (28))
-                                                         (Prims.of_int (29))
+                                                         (Prims.of_int (48))
                                                          (Prims.of_int (46)))))
                                                 (FStar_Sealed.seal
                                                    (Obj.magic
                                                       (FStar_Range.mk_range
                                                          "Pulse.Checker.Abs.fst"
-                                                         (Prims.of_int (28))
+                                                         (Prims.of_int (47))
                                                          (Prims.of_int (41))
-                                                         (Prims.of_int (59))
+                                                         (Prims.of_int (88))
                                                          (Prims.of_int (27)))))
                                                 (Obj.magic
                                                    (Pulse_Checker_Pure.check_universe
@@ -104,17 +467,17 @@ let (check_abs :
                                                                   (Obj.magic
                                                                     (FStar_Range.mk_range
                                                                     "Pulse.Checker.Abs.fst"
-                                                                    (Prims.of_int (30))
+                                                                    (Prims.of_int (49))
                                                                     (Prims.of_int (12))
-                                                                    (Prims.of_int (30))
+                                                                    (Prims.of_int (49))
                                                                     (Prims.of_int (19)))))
                                                                (FStar_Sealed.seal
                                                                   (Obj.magic
                                                                     (FStar_Range.mk_range
                                                                     "Pulse.Checker.Abs.fst"
-                                                                    (Prims.of_int (30))
+                                                                    (Prims.of_int (49))
                                                                     (Prims.of_int (22))
-                                                                    (Prims.of_int (59))
+                                                                    (Prims.of_int (88))
                                                                     (Prims.of_int (27)))))
                                                                (FStar_Tactics_Effect.lift_div_tac
                                                                   (fun uu___5
@@ -129,17 +492,17 @@ let (check_abs :
                                                                     (Obj.magic
                                                                     (FStar_Range.mk_range
                                                                     "Pulse.Checker.Abs.fst"
-                                                                    (Prims.of_int (31))
+                                                                    (Prims.of_int (50))
                                                                     (Prims.of_int (13))
-                                                                    (Prims.of_int (31))
+                                                                    (Prims.of_int (50))
                                                                     (Prims.of_int (22)))))
                                                                     (FStar_Sealed.seal
                                                                     (Obj.magic
                                                                     (FStar_Range.mk_range
                                                                     "Pulse.Checker.Abs.fst"
-                                                                    (Prims.of_int (31))
+                                                                    (Prims.of_int (50))
                                                                     (Prims.of_int (25))
-                                                                    (Prims.of_int (59))
+                                                                    (Prims.of_int (88))
                                                                     (Prims.of_int (27)))))
                                                                     (FStar_Tactics_Effect.lift_div_tac
                                                                     (fun
@@ -156,17 +519,49 @@ let (check_abs :
                                                                     (Obj.magic
                                                                     (FStar_Range.mk_range
                                                                     "Pulse.Checker.Abs.fst"
-                                                                    (Prims.of_int (32))
+                                                                    (Prims.of_int (51))
+                                                                    (Prims.of_int (14))
+                                                                    (Prims.of_int (51))
+                                                                    (Prims.of_int (50)))))
+                                                                    (FStar_Sealed.seal
+                                                                    (Obj.magic
+                                                                    (FStar_Range.mk_range
+                                                                    "Pulse.Checker.Abs.fst"
+                                                                    (Prims.of_int (51))
+                                                                    (Prims.of_int (53))
+                                                                    (Prims.of_int (88))
+                                                                    (Prims.of_int (27)))))
+                                                                    (FStar_Tactics_Effect.lift_div_tac
+                                                                    (fun
+                                                                    uu___5 ->
+                                                                    Pulse_Syntax_Pure.tm_var
+                                                                    {
+                                                                    Pulse_Syntax_Base.nm_index
+                                                                    = x;
+                                                                    Pulse_Syntax_Base.nm_ppname
+                                                                    = ppname
+                                                                    }))
+                                                                    (fun
+                                                                    uu___5 ->
+                                                                    (fun var
+                                                                    ->
+                                                                    Obj.magic
+                                                                    (FStar_Tactics_Effect.tac_bind
+                                                                    (FStar_Sealed.seal
+                                                                    (Obj.magic
+                                                                    (FStar_Range.mk_range
+                                                                    "Pulse.Checker.Abs.fst"
+                                                                    (Prims.of_int (52))
                                                                     (Prims.of_int (13))
-                                                                    (Prims.of_int (32))
+                                                                    (Prims.of_int (52))
                                                                     (Prims.of_int (38)))))
                                                                     (FStar_Sealed.seal
                                                                     (Obj.magic
                                                                     (FStar_Range.mk_range
                                                                     "Pulse.Checker.Abs.fst"
-                                                                    (Prims.of_int (32))
+                                                                    (Prims.of_int (52))
                                                                     (Prims.of_int (41))
-                                                                    (Prims.of_int (59))
+                                                                    (Prims.of_int (88))
                                                                     (Prims.of_int (27)))))
                                                                     (FStar_Tactics_Effect.lift_div_tac
                                                                     (fun
@@ -184,45 +579,67 @@ let (check_abs :
                                                                     (Obj.magic
                                                                     (FStar_Range.mk_range
                                                                     "Pulse.Checker.Abs.fst"
-                                                                    (Prims.of_int (34))
+                                                                    (Prims.of_int (54))
                                                                     (Prims.of_int (6))
-                                                                    (Prims.of_int (36))
-                                                                    (Prims.of_int (49)))))
+                                                                    (Prims.of_int (66))
+                                                                    (Prims.of_int (45)))))
                                                                     (FStar_Sealed.seal
                                                                     (Obj.magic
                                                                     (FStar_Range.mk_range
                                                                     "Pulse.Checker.Abs.fst"
-                                                                    (Prims.of_int (36))
                                                                     (Prims.of_int (52))
-                                                                    (Prims.of_int (59))
+                                                                    (Prims.of_int (41))
+                                                                    (Prims.of_int (88))
                                                                     (Prims.of_int (27)))))
-                                                                    (match pre_hint
-                                                                    with
-                                                                    | 
-                                                                    FStar_Pervasives_Native.None
-                                                                    ->
-                                                                    Obj.magic
-                                                                    (Obj.repr
-                                                                    (Pulse_Typing_Env.fail
-                                                                    g
-                                                                    FStar_Pervasives_Native.None
-                                                                    "Cannot typecheck an function without a precondition"))
-                                                                    | 
-                                                                    FStar_Pervasives_Native.Some
-                                                                    pre_hint1
-                                                                    ->
-                                                                    Obj.magic
-                                                                    (Obj.repr
                                                                     (FStar_Tactics_Effect.lift_div_tac
                                                                     (fun
                                                                     uu___5 ->
-                                                                    Pulse_Syntax_Naming.open_term_nv
-                                                                    pre_hint1
-                                                                    px))))
+                                                                    match c
+                                                                    with
+                                                                    | 
+                                                                    Pulse_Syntax_Base.C_Tot
+                                                                    {
+                                                                    Pulse_Syntax_Base.t
+                                                                    =
+                                                                    Pulse_Syntax_Base.Tm_Unknown;
+                                                                    Pulse_Syntax_Base.range1
+                                                                    = uu___6;_}
+                                                                    ->
+                                                                    (Pulse_Syntax_Base.tm_emp,
+                                                                    FStar_Pervasives_Native.None,
+                                                                    FStar_Pervasives_Native.None)
+                                                                    | 
+                                                                    Pulse_Syntax_Base.C_Tot
+                                                                    ty ->
+                                                                    (Pulse_Syntax_Base.tm_emp,
+                                                                    (FStar_Pervasives_Native.Some
+                                                                    (Pulse_Syntax_Naming.open_term_nv
+                                                                    ty px)),
+                                                                    FStar_Pervasives_Native.None)
+                                                                    | 
+                                                                    uu___6 ->
+                                                                    ((Pulse_Syntax_Naming.open_term_nv
+                                                                    (Pulse_Syntax_Base.comp_pre
+                                                                    c) px),
+                                                                    (FStar_Pervasives_Native.Some
+                                                                    (Pulse_Syntax_Naming.open_term_nv
+                                                                    (Pulse_Syntax_Base.comp_res
+                                                                    c) px)),
+                                                                    (FStar_Pervasives_Native.Some
+                                                                    (Pulse_Syntax_Naming.open_term'
+                                                                    (Pulse_Syntax_Base.comp_post
+                                                                    c) var
+                                                                    Prims.int_one)))))
                                                                     (fun
                                                                     uu___5 ->
                                                                     (fun
-                                                                    pre_opened
+                                                                    uu___5 ->
+                                                                    match uu___5
+                                                                    with
+                                                                    | 
+                                                                    (pre_opened,
+                                                                    ret_ty,
+                                                                    post_hint_body)
                                                                     ->
                                                                     Obj.magic
                                                                     (FStar_Tactics_Effect.tac_bind
@@ -230,27 +647,27 @@ let (check_abs :
                                                                     (Obj.magic
                                                                     (FStar_Range.mk_range
                                                                     "Pulse.Checker.Abs.fst"
-                                                                    (Prims.of_int (37))
+                                                                    (Prims.of_int (68))
                                                                     (Prims.of_int (39))
-                                                                    (Prims.of_int (37))
+                                                                    (Prims.of_int (68))
                                                                     (Prims.of_int (64)))))
                                                                     (FStar_Sealed.seal
                                                                     (Obj.magic
                                                                     (FStar_Range.mk_range
                                                                     "Pulse.Checker.Abs.fst"
-                                                                    (Prims.of_int (36))
-                                                                    (Prims.of_int (52))
-                                                                    (Prims.of_int (59))
+                                                                    (Prims.of_int (67))
+                                                                    (Prims.of_int (6))
+                                                                    (Prims.of_int (88))
                                                                     (Prims.of_int (27)))))
                                                                     (Obj.magic
                                                                     (Pulse_Checker_Pure.check_vprop
                                                                     g'
                                                                     pre_opened))
                                                                     (fun
-                                                                    uu___5 ->
+                                                                    uu___6 ->
                                                                     (fun
-                                                                    uu___5 ->
-                                                                    match uu___5
+                                                                    uu___6 ->
+                                                                    match uu___6
                                                                     with
                                                                     | 
                                                                     Prims.Mkdtuple2
@@ -263,26 +680,26 @@ let (check_abs :
                                                                     (Obj.magic
                                                                     (FStar_Range.mk_range
                                                                     "Pulse.Checker.Abs.fst"
-                                                                    (Prims.of_int (38))
+                                                                    (Prims.of_int (69))
                                                                     (Prims.of_int (14))
-                                                                    (Prims.of_int (38))
+                                                                    (Prims.of_int (69))
                                                                     (Prims.of_int (37)))))
                                                                     (FStar_Sealed.seal
                                                                     (Obj.magic
                                                                     (FStar_Range.mk_range
                                                                     "Pulse.Checker.Abs.fst"
-                                                                    (Prims.of_int (38))
+                                                                    (Prims.of_int (69))
                                                                     (Prims.of_int (40))
-                                                                    (Prims.of_int (59))
+                                                                    (Prims.of_int (88))
                                                                     (Prims.of_int (27)))))
                                                                     (FStar_Tactics_Effect.lift_div_tac
                                                                     (fun
-                                                                    uu___6 ->
+                                                                    uu___7 ->
                                                                     Pulse_Syntax_Naming.close_term
                                                                     pre_opened1
                                                                     x))
                                                                     (fun
-                                                                    uu___6 ->
+                                                                    uu___7 ->
                                                                     (fun pre1
                                                                     ->
                                                                     Obj.magic
@@ -291,111 +708,19 @@ let (check_abs :
                                                                     (Obj.magic
                                                                     (FStar_Range.mk_range
                                                                     "Pulse.Checker.Abs.fst"
-                                                                    (Prims.of_int (39))
-                                                                    (Prims.of_int (14))
-                                                                    (Prims.of_int (39))
-                                                                    (Prims.of_int (50)))))
-                                                                    (FStar_Sealed.seal
-                                                                    (Obj.magic
-                                                                    (FStar_Range.mk_range
-                                                                    "Pulse.Checker.Abs.fst"
-                                                                    (Prims.of_int (39))
-                                                                    (Prims.of_int (53))
-                                                                    (Prims.of_int (59))
-                                                                    (Prims.of_int (27)))))
-                                                                    (FStar_Tactics_Effect.lift_div_tac
-                                                                    (fun
-                                                                    uu___6 ->
-                                                                    Pulse_Syntax_Pure.tm_var
-                                                                    {
-                                                                    Pulse_Syntax_Base.nm_index
-                                                                    = x;
-                                                                    Pulse_Syntax_Base.nm_ppname
-                                                                    = ppname
-                                                                    }))
-                                                                    (fun
-                                                                    uu___6 ->
-                                                                    (fun var
-                                                                    ->
-                                                                    Obj.magic
-                                                                    (FStar_Tactics_Effect.tac_bind
-                                                                    (FStar_Sealed.seal
-                                                                    (Obj.magic
-                                                                    (FStar_Range.mk_range
-                                                                    "Pulse.Checker.Abs.fst"
-                                                                    (Prims.of_int (40))
-                                                                    (Prims.of_int (17))
-                                                                    (Prims.of_int (40))
-                                                                    (Prims.of_int (44)))))
-                                                                    (FStar_Sealed.seal
-                                                                    (Obj.magic
-                                                                    (FStar_Range.mk_range
-                                                                    "Pulse.Checker.Abs.fst"
-                                                                    (Prims.of_int (40))
-                                                                    (Prims.of_int (47))
-                                                                    (Prims.of_int (59))
-                                                                    (Prims.of_int (27)))))
-                                                                    (FStar_Tactics_Effect.lift_div_tac
-                                                                    (fun
-                                                                    uu___6 ->
-                                                                    Pulse_Syntax_Naming.open_term_opt'
-                                                                    ret_ty
-                                                                    var
-                                                                    Prims.int_zero))
-                                                                    (fun
-                                                                    uu___6 ->
-                                                                    (fun
-                                                                    ret_ty1
-                                                                    ->
-                                                                    Obj.magic
-                                                                    (FStar_Tactics_Effect.tac_bind
-                                                                    (FStar_Sealed.seal
-                                                                    (Obj.magic
-                                                                    (FStar_Range.mk_range
-                                                                    "Pulse.Checker.Abs.fst"
-                                                                    (Prims.of_int (41))
-                                                                    (Prims.of_int (25))
-                                                                    (Prims.of_int (41))
-                                                                    (Prims.of_int (60)))))
-                                                                    (FStar_Sealed.seal
-                                                                    (Obj.magic
-                                                                    (FStar_Range.mk_range
-                                                                    "Pulse.Checker.Abs.fst"
-                                                                    (Prims.of_int (41))
-                                                                    (Prims.of_int (63))
-                                                                    (Prims.of_int (59))
-                                                                    (Prims.of_int (27)))))
-                                                                    (FStar_Tactics_Effect.lift_div_tac
-                                                                    (fun
-                                                                    uu___6 ->
-                                                                    Pulse_Syntax_Naming.open_term_opt'
-                                                                    post_hint_body
-                                                                    var
-                                                                    Prims.int_one))
-                                                                    (fun
-                                                                    uu___6 ->
-                                                                    (fun
-                                                                    post_hint_body1
-                                                                    ->
-                                                                    Obj.magic
-                                                                    (FStar_Tactics_Effect.tac_bind
-                                                                    (FStar_Sealed.seal
-                                                                    (Obj.magic
-                                                                    (FStar_Range.mk_range
-                                                                    "Pulse.Checker.Abs.fst"
-                                                                    (Prims.of_int (43))
+                                                                    (Prims.of_int (71))
                                                                     (Prims.of_int (6))
-                                                                    (Prims.of_int (50))
+                                                                    (Prims.of_int (78))
                                                                     (Prims.of_int (29)))))
                                                                     (FStar_Sealed.seal
                                                                     (Obj.magic
                                                                     (FStar_Range.mk_range
                                                                     "Pulse.Checker.Abs.fst"
-                                                                    (Prims.of_int (51))
+                                                                    (Prims.of_int (79))
                                                                     (Prims.of_int (6))
-                                                                    (Prims.of_int (59))
+                                                                    (Prims.of_int (88))
                                                                     (Prims.of_int (27)))))
-                                                                    (match post_hint_body1
+                                                                    (match post_hint_body
                                                                     with
                                                                     | 
                                                                     FStar_Pervasives_Native.None
@@ -404,7 +729,7 @@ let (check_abs :
                                                                     (Obj.repr
                                                                     (FStar_Tactics_Effect.lift_div_tac
                                                                     (fun
-                                                                    uu___6 ->
+                                                                    uu___7 ->
                                                                     FStar_Pervasives_Native.None)))
                                                                     | 
                                                                     FStar_Pervasives_Native.Some
@@ -416,35 +741,35 @@ let (check_abs :
                                                                     (Obj.magic
                                                                     (FStar_Range.mk_range
                                                                     "Pulse.Checker.Abs.fst"
-                                                                    (Prims.of_int (48))
+                                                                    (Prims.of_int (76))
                                                                     (Prims.of_int (12))
-                                                                    (Prims.of_int (48))
+                                                                    (Prims.of_int (76))
                                                                     (Prims.of_int (103)))))
                                                                     (FStar_Sealed.seal
                                                                     (Obj.magic
                                                                     (FStar_Range.mk_range
                                                                     "Pulse.Checker.Abs.fst"
-                                                                    (Prims.of_int (50))
+                                                                    (Prims.of_int (78))
                                                                     (Prims.of_int (8))
-                                                                    (Prims.of_int (50))
+                                                                    (Prims.of_int (78))
                                                                     (Prims.of_int (29)))))
                                                                     (Obj.magic
                                                                     (Pulse_Checker_Common.intro_post_hint
                                                                     (Pulse_Checker_Pure.push_context
                                                                     "post_hint_typing"
                                                                     range g')
-                                                                    ret_ty1
+                                                                    ret_ty
                                                                     post))
                                                                     (fun
                                                                     post_hint_typing
                                                                     ->
                                                                     FStar_Tactics_Effect.lift_div_tac
                                                                     (fun
-                                                                    uu___6 ->
+                                                                    uu___7 ->
                                                                     FStar_Pervasives_Native.Some
                                                                     post_hint_typing)))))
                                                                     (fun
-                                                                    uu___6 ->
+                                                                    uu___7 ->
                                                                     (fun post
                                                                     ->
                                                                     Obj.magic
@@ -453,17 +778,17 @@ let (check_abs :
                                                                     (Obj.magic
                                                                     (FStar_Range.mk_range
                                                                     "Pulse.Checker.Abs.fst"
-                                                                    (Prims.of_int (52))
+                                                                    (Prims.of_int (80))
                                                                     (Prims.of_int (43))
-                                                                    (Prims.of_int (52))
+                                                                    (Prims.of_int (80))
                                                                     (Prims.of_int (104)))))
                                                                     (FStar_Sealed.seal
                                                                     (Obj.magic
                                                                     (FStar_Range.mk_range
                                                                     "Pulse.Checker.Abs.fst"
-                                                                    (Prims.of_int (51))
+                                                                    (Prims.of_int (79))
                                                                     (Prims.of_int (6))
-                                                                    (Prims.of_int (59))
+                                                                    (Prims.of_int (88))
                                                                     (Prims.of_int (27)))))
                                                                     (Obj.magic
                                                                     (check g'
@@ -472,11 +797,10 @@ let (check_abs :
                                                                     pre_opened1
                                                                     () post))
                                                                     (fun
-                                                                    uu___6 ->
-                                                                    FStar_Tactics_Effect.lift_div_tac
+                                                                    uu___7 ->
                                                                     (fun
                                                                     uu___7 ->
-                                                                    match uu___6
+                                                                    match uu___7
                                                                     with
                                                                     | 
                                                                     FStar_Pervasives.Mkdtuple3
@@ -484,6 +808,34 @@ let (check_abs :
                                                                     c_body,
                                                                     body_typing)
                                                                     ->
+                                                                    Obj.magic
+                                                                    (FStar_Tactics_Effect.tac_bind
+                                                                    (FStar_Sealed.seal
+                                                                    (Obj.magic
+                                                                    (FStar_Range.mk_range
+                                                                    "Pulse.Checker.Abs.fst"
+                                                                    (Prims.of_int (81))
+                                                                    (Prims.of_int (4))
+                                                                    (Prims.of_int (81))
+                                                                    (Prims.of_int (51)))))
+                                                                    (FStar_Sealed.seal
+                                                                    (Obj.magic
+                                                                    (FStar_Range.mk_range
+                                                                    "Pulse.Checker.Abs.fst"
+                                                                    (Prims.of_int (88))
+                                                                    (Prims.of_int (4))
+                                                                    (Prims.of_int (88))
+                                                                    (Prims.of_int (27)))))
+                                                                    (Obj.magic
+                                                                    (check_effect_annotation
+                                                                    g'
+                                                                    body'.Pulse_Syntax_Base.range2
+                                                                    c c_body))
+                                                                    (fun
+                                                                    uu___8 ->
+                                                                    FStar_Tactics_Effect.lift_div_tac
+                                                                    (fun
+                                                                    uu___9 ->
                                                                     FStar_Pervasives.Mkdtuple3
                                                                     ((Pulse_Typing.wr
                                                                     (Pulse_Syntax_Base.Tm_Abs
@@ -498,19 +850,14 @@ let (check_abs :
                                                                     };
                                                                     Pulse_Syntax_Base.q
                                                                     = qual;
-                                                                    Pulse_Syntax_Base.pre1
+                                                                    Pulse_Syntax_Base.ascription
                                                                     =
-                                                                    FStar_Pervasives_Native.None;
+                                                                    (Pulse_Syntax_Naming.close_comp
+                                                                    c_body x);
                                                                     Pulse_Syntax_Base.body
                                                                     =
                                                                     (Pulse_Syntax_Naming.close_st_term
-                                                                    body' x);
-                                                                    Pulse_Syntax_Base.ret_ty
-                                                                    =
-                                                                    FStar_Pervasives_Native.None;
-                                                                    Pulse_Syntax_Base.post1
-                                                                    =
-                                                                    FStar_Pervasives_Native.None
+                                                                    body' x)
                                                                     })),
                                                                     (Pulse_Syntax_Base.C_Tot
                                                                     (Pulse_Syntax_Pure.tm_arrow
@@ -536,10 +883,9 @@ let (check_abs :
                                                                     c_body,
                                                                     (),
                                                                     body_typing)))))))
-                                                                    uu___6)))
-                                                                    uu___6)))
-                                                                    uu___6)))
-                                                                    uu___6)))
+                                                                    uu___7)))
+                                                                    uu___7)))
+                                                                    uu___7)))
                                                                     uu___6)))
                                                                     uu___5)))
                                                                     uu___5)))
