pulse/src/ocaml/plugin/generated/Pulse_Syntax_Printer.ml
@@ -1539,21 +1539,20 @@ let rec (st_term_to_string' :
                             (fun uu___2 -> uu___1 uu___)))) uu___)
       | Pulse_Syntax_Base.Tm_Abs
           { Pulse_Syntax_Base.b = b; Pulse_Syntax_Base.q = q;
-            Pulse_Syntax_Base.pre1 = pre; Pulse_Syntax_Base.body = body;
-            Pulse_Syntax_Base.ret_ty = ret_ty;
-            Pulse_Syntax_Base.post1 = post;_}
+            Pulse_Syntax_Base.ascription = c;
+            Pulse_Syntax_Base.body = body;_}
           ->
           FStar_Tactics_Effect.tac_bind
             (FStar_Sealed.seal
                (Obj.magic
                   (FStar_Range.mk_range "Pulse.Syntax.Printer.fst"
-                     (Prims.of_int (165)) (Prims.of_int (14))
-                     (Prims.of_int (165)) (Prims.of_int (54)))))
+                     (Prims.of_int (163)) (Prims.of_int (14))
+                     (Prims.of_int (163)) (Prims.of_int (54)))))
             (FStar_Sealed.seal
                (Obj.magic
                   (FStar_Range.mk_range "Pulse.Syntax.Printer.fst"
                      (Prims.of_int (158)) (Prims.of_int (6))
-                     (Prims.of_int (165)) (Prims.of_int (54)))))
+                     (Prims.of_int (163)) (Prims.of_int (54)))))
             (Obj.magic (st_term_to_string' (indent level) body))
             (fun uu___ ->
                (fun uu___ ->
@@ -1563,12 +1562,12 @@ let rec (st_term_to_string' :
                           (Obj.magic
                              (FStar_Range.mk_range "Pulse.Syntax.Printer.fst"
                                 (Prims.of_int (158)) (Prims.of_int (6))
-                                (Prims.of_int (165)) (Prims.of_int (54)))))
+                                (Prims.of_int (163)) (Prims.of_int (54)))))
                        (FStar_Sealed.seal
                           (Obj.magic
                              (FStar_Range.mk_range "Pulse.Syntax.Printer.fst"
                                 (Prims.of_int (158)) (Prims.of_int (6))
-                                (Prims.of_int (165)) (Prims.of_int (54)))))
+                                (Prims.of_int (163)) (Prims.of_int (54)))))
                        (Obj.magic
                           (FStar_Tactics_Effect.tac_bind
                              (FStar_Sealed.seal
@@ -1576,14 +1575,14 @@ let rec (st_term_to_string' :
                                    (FStar_Range.mk_range
                                       "Pulse.Syntax.Printer.fst"
                                       (Prims.of_int (158)) (Prims.of_int (6))
-                                      (Prims.of_int (165))
+                                      (Prims.of_int (163))
                                       (Prims.of_int (54)))))
                              (FStar_Sealed.seal
                                 (Obj.magic
                                    (FStar_Range.mk_range
                                       "Pulse.Syntax.Printer.fst"
                                       (Prims.of_int (158)) (Prims.of_int (6))
-                                      (Prims.of_int (165))
+                                      (Prims.of_int (163))
                                       (Prims.of_int (54)))))
                              (Obj.magic
                                 (FStar_Tactics_Effect.tac_bind
@@ -1591,19 +1590,19 @@ let rec (st_term_to_string' :
                                       (Obj.magic
                                          (FStar_Range.mk_range
                                             "Pulse.Syntax.Printer.fst"
-                                            (Prims.of_int (163))
+                                            (Prims.of_int (161))
                                             (Prims.of_int (14))
-                                            (Prims.of_int (163))
-                                            (Prims.of_int (39)))))
+                                            (Prims.of_int (161))
+                                            (Prims.of_int (32)))))
                                    (FStar_Sealed.seal
                                       (Obj.magic
                                          (FStar_Range.mk_range
                                             "Pulse.Syntax.Printer.fst"
                                             (Prims.of_int (158))
                                             (Prims.of_int (6))
-                                            (Prims.of_int (165))
+                                            (Prims.of_int (163))
                                             (Prims.of_int (54)))))
-                                   (Obj.magic (term_opt_to_string post))
+                                   (Obj.magic (comp_to_string c))
                                    (fun uu___1 ->
                                       (fun uu___1 ->
                                          Obj.magic
@@ -1614,7 +1613,7 @@ let rec (st_term_to_string' :
                                                        "Pulse.Syntax.Printer.fst"
                                                        (Prims.of_int (158))
                                                        (Prims.of_int (6))
-                                                       (Prims.of_int (165))
+                                                       (Prims.of_int (163))
                                                        (Prims.of_int (54)))))
                                               (FStar_Sealed.seal
                                                  (Obj.magic
@@ -1622,7 +1621,7 @@ let rec (st_term_to_string' :
                                                        "Pulse.Syntax.Printer.fst"
                                                        (Prims.of_int (158))
                                                        (Prims.of_int (6))
-                                                       (Prims.of_int (165))
+                                                       (Prims.of_int (163))
                                                        (Prims.of_int (54)))))
                                               (Obj.magic
                                                  (FStar_Tactics_Effect.tac_bind
@@ -1630,119 +1629,29 @@ let rec (st_term_to_string' :
                                                        (Obj.magic
                                                           (FStar_Range.mk_range
                                                              "Pulse.Syntax.Printer.fst"
-                                                             (Prims.of_int (162))
+                                                             (Prims.of_int (160))
                                                              (Prims.of_int (14))
-                                                             (Prims.of_int (162))
-                                                             (Prims.of_int (41)))))
+                                                             (Prims.of_int (160))
+                                                             (Prims.of_int (34)))))
                                                     (FStar_Sealed.seal
                                                        (Obj.magic
                                                           (FStar_Range.mk_range
-                                                             "Pulse.Syntax.Printer.fst"
-                                                             (Prims.of_int (158))
-                                                             (Prims.of_int (6))
-                                                             (Prims.of_int (165))
-                                                             (Prims.of_int (54)))))
+                                                             "FStar.Printf.fst"
+                                                             (Prims.of_int (121))
+                                                             (Prims.of_int (8))
+                                                             (Prims.of_int (123))
+                                                             (Prims.of_int (44)))))
                                                     (Obj.magic
-                                                       (term_opt_to_string
-                                                          ret_ty))
+                                                       (binder_to_string b))
                                                     (fun uu___2 ->
-                                                       (fun uu___2 ->
-                                                          Obj.magic
-                                                            (FStar_Tactics_Effect.tac_bind
-                                                               (FStar_Sealed.seal
-                                                                  (Obj.magic
-                                                                    (FStar_Range.mk_range
-                                                                    "Pulse.Syntax.Printer.fst"
-                                                                    (Prims.of_int (158))
-                                                                    (Prims.of_int (6))
-                                                                    (Prims.of_int (165))
-                                                                    (Prims.of_int (54)))))
-                                                               (FStar_Sealed.seal
-                                                                  (Obj.magic
-                                                                    (FStar_Range.mk_range
-                                                                    "Pulse.Syntax.Printer.fst"
-                                                                    (Prims.of_int (158))
-                                                                    (Prims.of_int (6))
-                                                                    (Prims.of_int (165))
-                                                                    (Prims.of_int (54)))))
-                                                               (Obj.magic
-                                                                  (FStar_Tactics_Effect.tac_bind
-                                                                    (FStar_Sealed.seal
-                                                                    (Obj.magic
-                                                                    (FStar_Range.mk_range
-                                                                    "Pulse.Syntax.Printer.fst"
-                                                                    (Prims.of_int (161))
-                                                                    (Prims.of_int (14))
-                                                                    (Prims.of_int (161))
-                                                                    (Prims.of_int (38)))))
-                                                                    (FStar_Sealed.seal
-                                                                    (Obj.magic
-                                                                    (FStar_Range.mk_range
-                                                                    "Pulse.Syntax.Printer.fst"
-                                                                    (Prims.of_int (158))
-                                                                    (Prims.of_int (6))
-                                                                    (Prims.of_int (165))
-                                                                    (Prims.of_int (54)))))
-                                                                    (Obj.magic
-                                                                    (term_opt_to_string
-                                                                    pre))
-                                                                    (fun
-                                                                    uu___3 ->
-                                                                    (fun
-                                                                    uu___3 ->
-                                                                    Obj.magic
-                                                                    (FStar_Tactics_Effect.tac_bind
-                                                                    (FStar_Sealed.seal
-                                                                    (Obj.magic
-                                                                    (FStar_Range.mk_range
-                                                                    "Pulse.Syntax.Printer.fst"
-                                                                    (Prims.of_int (158))
-                                                                    (Prims.of_int (6))
-                                                                    (Prims.of_int (165))
-                                                                    (Prims.of_int (54)))))
-                                                                    (FStar_Sealed.seal
-                                                                    (Obj.magic
-                                                                    (FStar_Range.mk_range
-                                                                    "Pulse.Syntax.Printer.fst"
-                                                                    (Prims.of_int (158))
-                                                                    (Prims.of_int (6))
-                                                                    (Prims.of_int (165))
-                                                                    (Prims.of_int (54)))))
-                                                                    (Obj.magic
-                                                                    (FStar_Tactics_Effect.tac_bind
-                                                                    (FStar_Sealed.seal
-                                                                    (Obj.magic
-                                                                    (FStar_Range.mk_range
-                                                                    "Pulse.Syntax.Printer.fst"
-                                                                    (Prims.of_int (160))
-                                                                    (Prims.of_int (14))
-                                                                    (Prims.of_int (160))
-                                                                    (Prims.of_int (34)))))
-                                                                    (FStar_Sealed.seal
-                                                                    (Obj.magic
-                                                                    (FStar_Range.mk_range
-                                                                    "FStar.Printf.fst"
-                                                                    (Prims.of_int (121))
-                                                                    (Prims.of_int (8))
-                                                                    (Prims.of_int (123))
-                                                                    (Prims.of_int (44)))))
-                                                                    (Obj.magic
-                                                                    (binder_to_string
-                                                                    b))
-                                                                    (fun
-                                                                    uu___4 ->
-                                                                    FStar_Tactics_Effect.lift_div_tac
-                                                                    (fun
-                                                                    uu___5 ->
-                                                                    fun x ->
-                                                                    fun x1 ->
-                                                                    fun x2 ->
-                                                                    fun x3 ->
-                                                                    fun x4 ->
+                                                       FStar_Tactics_Effect.lift_div_tac
+                                                         (fun uu___3 ->
+                                                            fun x ->
+                                                              fun x1 ->
+                                                                fun x2 ->
+                                                                  Prims.strcat
+                                                                    (
                                                                     Prims.strcat
-                                                                    (Prims.strcat
-                                                                    (Prims.strcat
-                                                                    (Prims.strcat
                                                                     (Prims.strcat
                                                                     (Prims.strcat
                                                                     (Prims.strcat
@@ -1751,37 +1660,16 @@ let rec (st_term_to_string' :
                                                                     (qual_to_string
                                                                     q) ""))
                                                                     (Prims.strcat
-                                                                    uu___4
-                                                                    ")\nrequires\n"))
+                                                                    uu___2
+                                                                    ")\n"))
                                                                     (Prims.strcat
                                                                     x
-                                                                    "\nreturns "))
-                                                                    (Prims.strcat
-                                                                    x1
-                                                                    "\nensures\n"))
-                                                                    (Prims.strcat
-                                                                    x2
                                                                     "\n {\n"))
                                                                     (Prims.strcat
-                                                                    x3 ""))
-                                                                    (Prims.strcat
-                                                                    x4 "\n}")))))
-                                                                    (fun
-                                                                    uu___4 ->
-                                                                    FStar_Tactics_Effect.lift_div_tac
-                                                                    (fun
-                                                                    uu___5 ->
-                                                                    uu___4
-                                                                    uu___3))))
-                                                                    uu___3)))
-                                                               (fun uu___3 ->
-                                                                  FStar_Tactics_Effect.lift_div_tac
+                                                                    x1 ""))
                                                                     (
-                                                                    fun
-                                                                    uu___4 ->
-                                                                    uu___3
-                                                                    uu___2))))
-                                                         uu___2)))
+                                                                    Prims.strcat
+                                                                    x2 "\n}")))))
                                               (fun uu___2 ->
                                                  FStar_Tactics_Effect.lift_div_tac
                                                    (fun uu___3 ->
@@ -1796,31 +1684,31 @@ let rec (st_term_to_string' :
       | Pulse_Syntax_Base.Tm_If
           { Pulse_Syntax_Base.b1 = b; Pulse_Syntax_Base.then_ = then_;
             Pulse_Syntax_Base.else_ = else_;
-            Pulse_Syntax_Base.post2 = uu___;_}
+            Pulse_Syntax_Base.post1 = uu___;_}
           ->
           FStar_Tactics_Effect.tac_bind
             (FStar_Sealed.seal
                (Obj.magic
                   (FStar_Range.mk_range "Pulse.Syntax.Printer.fst"
-                     (Prims.of_int (168)) (Prims.of_int (6))
-                     (Prims.of_int (178)) (Prims.of_int (13)))))
+                     (Prims.of_int (166)) (Prims.of_int (6))
+                     (Prims.of_int (176)) (Prims.of_int (13)))))
             (FStar_Sealed.seal
                (Obj.magic
                   (FStar_Range.mk_range "Pulse.Syntax.Printer.fst"
-                     (Prims.of_int (168)) (Prims.of_int (6))
-                     (Prims.of_int (178)) (Prims.of_int (13)))))
+                     (Prims.of_int (166)) (Prims.of_int (6))
+                     (Prims.of_int (176)) (Prims.of_int (13)))))
             (Obj.magic
                (FStar_Tactics_Effect.tac_bind
                   (FStar_Sealed.seal
                      (Obj.magic
                         (FStar_Range.mk_range "Pulse.Syntax.Printer.fst"
-                           (Prims.of_int (177)) (Prims.of_int (8))
-                           (Prims.of_int (177)) (Prims.of_int (49)))))
+                           (Prims.of_int (175)) (Prims.of_int (8))
+                           (Prims.of_int (175)) (Prims.of_int (49)))))
                   (FStar_Sealed.seal
                      (Obj.magic
                         (FStar_Range.mk_range "Pulse.Syntax.Printer.fst"
-                           (Prims.of_int (168)) (Prims.of_int (6))
-                           (Prims.of_int (178)) (Prims.of_int (13)))))
+                           (Prims.of_int (166)) (Prims.of_int (6))
+                           (Prims.of_int (176)) (Prims.of_int (13)))))
                   (Obj.magic (st_term_to_string' (indent level) else_))
                   (fun uu___1 ->
                      (fun uu___1 ->
@@ -1830,15 +1718,15 @@ let rec (st_term_to_string' :
                                 (Obj.magic
                                    (FStar_Range.mk_range
                                       "Pulse.Syntax.Printer.fst"
-                                      (Prims.of_int (168)) (Prims.of_int (6))
-                                      (Prims.of_int (178))
+                                      (Prims.of_int (166)) (Prims.of_int (6))
+                                      (Prims.of_int (176))
                                       (Prims.of_int (13)))))
                              (FStar_Sealed.seal
                                 (Obj.magic
                                    (FStar_Range.mk_range
                                       "Pulse.Syntax.Printer.fst"
-                                      (Prims.of_int (168)) (Prims.of_int (6))
-                                      (Prims.of_int (178))
+                                      (Prims.of_int (166)) (Prims.of_int (6))
+                                      (Prims.of_int (176))
                                       (Prims.of_int (13)))))
                              (Obj.magic
                                 (FStar_Tactics_Effect.tac_bind
@@ -1846,17 +1734,17 @@ let rec (st_term_to_string' :
                                       (Obj.magic
                                          (FStar_Range.mk_range
                                             "Pulse.Syntax.Printer.fst"
-                                            (Prims.of_int (168))
+                                            (Prims.of_int (166))
                                             (Prims.of_int (6))
-                                            (Prims.of_int (178))
+                                            (Prims.of_int (176))
                                             (Prims.of_int (13)))))
                                    (FStar_Sealed.seal
                                       (Obj.magic
                                          (FStar_Range.mk_range
                                             "Pulse.Syntax.Printer.fst"
-                                            (Prims.of_int (168))
+                                            (Prims.of_int (166))
                                             (Prims.of_int (6))
-                                            (Prims.of_int (178))
+                                            (Prims.of_int (176))
                                             (Prims.of_int (13)))))
                                    (Obj.magic
                                       (FStar_Tactics_Effect.tac_bind
@@ -1864,17 +1752,17 @@ let rec (st_term_to_string' :
                                             (Obj.magic
                                                (FStar_Range.mk_range
                                                   "Pulse.Syntax.Printer.fst"
-                                                  (Prims.of_int (168))
+                                                  (Prims.of_int (166))
                                                   (Prims.of_int (6))
-                                                  (Prims.of_int (178))
+                                                  (Prims.of_int (176))
                                                   (Prims.of_int (13)))))
                                          (FStar_Sealed.seal
                                             (Obj.magic
                                                (FStar_Range.mk_range
                                                   "Pulse.Syntax.Printer.fst"
-                                                  (Prims.of_int (168))
+                                                  (Prims.of_int (166))
                                                   (Prims.of_int (6))
-                                                  (Prims.of_int (178))
+                                                  (Prims.of_int (176))
                                                   (Prims.of_int (13)))))
                                          (Obj.magic
                                             (FStar_Tactics_Effect.tac_bind
@@ -1882,17 +1770,17 @@ let rec (st_term_to_string' :
                                                   (Obj.magic
                                                      (FStar_Range.mk_range
                                                         "Pulse.Syntax.Printer.fst"
-                                                        (Prims.of_int (168))
+                                                        (Prims.of_int (166))
                                                         (Prims.of_int (6))
-                                                        (Prims.of_int (178))
+                                                        (Prims.of_int (176))
                                                         (Prims.of_int (13)))))
                                                (FStar_Sealed.seal
                                                   (Obj.magic
                                                      (FStar_Range.mk_range
                                                         "Pulse.Syntax.Printer.fst"
-                                                        (Prims.of_int (168))
+                                                        (Prims.of_int (166))
                                                         (Prims.of_int (6))
-                                                        (Prims.of_int (178))
+                                                        (Prims.of_int (176))
                                                         (Prims.of_int (13)))))
                                                (Obj.magic
                                                   (FStar_Tactics_Effect.tac_bind
@@ -1900,17 +1788,17 @@ let rec (st_term_to_string' :
                                                         (Obj.magic
                                                            (FStar_Range.mk_range
                                                               "Pulse.Syntax.Printer.fst"
-                                                              (Prims.of_int (168))
+                                                              (Prims.of_int (166))
                                                               (Prims.of_int (6))
-                                                              (Prims.of_int (178))
+                                                              (Prims.of_int (176))
                                                               (Prims.of_int (13)))))
                                                      (FStar_Sealed.seal
                                                         (Obj.magic
                                                            (FStar_Range.mk_range
                                                               "Pulse.Syntax.Printer.fst"
-                                                              (Prims.of_int (168))
+                                                              (Prims.of_int (166))
                                                               (Prims.of_int (6))
-                                                              (Prims.of_int (178))
+                                                              (Prims.of_int (176))
                                                               (Prims.of_int (13)))))
                                                      (Obj.magic
                                                         (FStar_Tactics_Effect.tac_bind
@@ -1918,17 +1806,17 @@ let rec (st_term_to_string' :
                                                               (Obj.magic
                                                                  (FStar_Range.mk_range
                                                                     "Pulse.Syntax.Printer.fst"
-                                                                    (Prims.of_int (172))
+                                                                    (Prims.of_int (170))
                                                                     (Prims.of_int (8))
-                                                                    (Prims.of_int (172))
+                                                                    (Prims.of_int (170))
                                                                     (Prims.of_int (49)))))
                                                            (FStar_Sealed.seal
                                                               (Obj.magic
                                                                  (FStar_Range.mk_range
                                                                     "Pulse.Syntax.Printer.fst"
-                                                                    (Prims.of_int (168))
+                                                                    (Prims.of_int (166))
                                                                     (Prims.of_int (6))
-                                                                    (Prims.of_int (178))
+                                                                    (Prims.of_int (176))
                                                                     (Prims.of_int (13)))))
                                                            (Obj.magic
                                                               (st_term_to_string'
@@ -1943,35 +1831,17 @@ let rec (st_term_to_string' :
                                                                     (Obj.magic
                                                                     (FStar_Range.mk_range
                                                                     "Pulse.Syntax.Printer.fst"
-                                                                    (Prims.of_int (168))
+                                                                    (Prims.of_int (166))
                                                                     (Prims.of_int (6))
-                                                                    (Prims.of_int (178))
+                                                                    (Prims.of_int (176))
                                                                     (Prims.of_int (13)))))
                                                                     (FStar_Sealed.seal
                                                                     (Obj.magic
                                                                     (FStar_Range.mk_range
                                                                     "Pulse.Syntax.Printer.fst"
-                                                                    (Prims.of_int (168))
+                                                                    (Prims.of_int (166))
                                                                     (Prims.of_int (6))
-                                                                    (Prims.of_int (178))
-                                                                    (Prims.of_int (13)))))
-                                                                    (Obj.magic
-                                                                    (FStar_Tactics_Effect.tac_bind
-                                                                    (FStar_Sealed.seal
-                                                                    (Obj.magic
-                                                                    (FStar_Range.mk_range
-                                                                    "Pulse.Syntax.Printer.fst"
-                                                                    (Prims.of_int (168))
-                                                                    (Prims.of_int (6))
-                                                                    (Prims.of_int (178))
-                                                                    (Prims.of_int (13)))))
-                                                                    (FStar_Sealed.seal
-                                                                    (Obj.magic
-                                                                    (FStar_Range.mk_range
-                                                                    "Pulse.Syntax.Printer.fst"
-                                                                    (Prims.of_int (168))
-                                                                    (Prims.of_int (6))
-                                                                    (Prims.of_int (178))
+                                                                    (Prims.of_int (176))
                                                                     (Prims.of_int (13)))))
                                                                     (Obj.magic
                                                                     (FStar_Tactics_Effect.tac_bind
@@ -1979,17 +1849,17 @@ let rec (st_term_to_string' :
                                                                     (Obj.magic
                                                                     (FStar_Range.mk_range
                                                                     "Pulse.Syntax.Printer.fst"
-                                                                    (Prims.of_int (168))
+                                                                    (Prims.of_int (166))
                                                                     (Prims.of_int (6))
-                                                                    (Prims.of_int (178))
+                                                                    (Prims.of_int (176))
                                                                     (Prims.of_int (13)))))
                                                                     (FStar_Sealed.seal
                                                                     (Obj.magic
                                                                     (FStar_Range.mk_range
                                                                     "Pulse.Syntax.Printer.fst"
-                                                                    (Prims.of_int (168))
+                                                                    (Prims.of_int (166))
                                                                     (Prims.of_int (6))
-                                                                    (Prims.of_int (178))
+                                                                    (Prims.of_int (176))
                                                                     (Prims.of_int (13)))))
                                                                     (Obj.magic
                                                                     (FStar_Tactics_Effect.tac_bind
@@ -1997,9 +1867,27 @@ let rec (st_term_to_string' :
                                                                     (Obj.magic
                                                                     (FStar_Range.mk_range
                                                                     "Pulse.Syntax.Printer.fst"
-                                                                    (Prims.of_int (169))
+                                                                    (Prims.of_int (166))
+                                                                    (Prims.of_int (6))
+                                                                    (Prims.of_int (176))
+                                                                    (Prims.of_int (13)))))
+                                                                    (FStar_Sealed.seal
+                                                                    (Obj.magic
+                                                                    (FStar_Range.mk_range
+                                                                    "Pulse.Syntax.Printer.fst"
+                                                                    (Prims.of_int (166))
+                                                                    (Prims.of_int (6))
+                                                                    (Prims.of_int (176))
+                                                                    (Prims.of_int (13)))))
+                                                                    (Obj.magic
+                                                                    (FStar_Tactics_Effect.tac_bind
+                                                                    (FStar_Sealed.seal
+                                                                    (Obj.magic
+                                                                    (FStar_Range.mk_range
+                                                                    "Pulse.Syntax.Printer.fst"
+                                                                    (Prims.of_int (167))
                                                                     (Prims.of_int (8))
-                                                                    (Prims.of_int (169))
+                                                                    (Prims.of_int (167))
                                                                     (Prims.of_int (26)))))
                                                                     (FStar_Sealed.seal
                                                                     (Obj.magic
@@ -2109,8 +1997,8 @@ let rec (st_term_to_string' :
             (FStar_Sealed.seal
                (Obj.magic
                   (FStar_Range.mk_range "Pulse.Syntax.Printer.fst"
-                     (Prims.of_int (183)) (Prims.of_int (8))
-                     (Prims.of_int (183)) (Prims.of_int (42)))))
+                     (Prims.of_int (181)) (Prims.of_int (8))
+                     (Prims.of_int (181)) (Prims.of_int (42)))))
             (FStar_Sealed.seal
                (Obj.magic
                   (FStar_Range.mk_range "prims.fst" (Prims.of_int (590))
@@ -2129,8 +2017,8 @@ let rec (st_term_to_string' :
             (FStar_Sealed.seal
                (Obj.magic
                   (FStar_Range.mk_range "Pulse.Syntax.Printer.fst"
-                     (Prims.of_int (187)) (Prims.of_int (8))
-                     (Prims.of_int (187)) (Prims.of_int (26)))))
+                     (Prims.of_int (185)) (Prims.of_int (8))
+                     (Prims.of_int (185)) (Prims.of_int (26)))))
             (FStar_Sealed.seal
                (Obj.magic
                   (FStar_Range.mk_range "prims.fst" (Prims.of_int (590))
@@ -2149,13 +2037,13 @@ let rec (st_term_to_string' :
             (FStar_Sealed.seal
                (Obj.magic
                   (FStar_Range.mk_range "Pulse.Syntax.Printer.fst"
-                     (Prims.of_int (194)) (Prims.of_int (8))
-                     (Prims.of_int (194)) (Prims.of_int (43)))))
+                     (Prims.of_int (192)) (Prims.of_int (8))
+                     (Prims.of_int (192)) (Prims.of_int (43)))))
             (FStar_Sealed.seal
                (Obj.magic
                   (FStar_Range.mk_range "Pulse.Syntax.Printer.fst"
-                     (Prims.of_int (190)) (Prims.of_int (6))
-                     (Prims.of_int (194)) (Prims.of_int (43)))))
+                     (Prims.of_int (188)) (Prims.of_int (6))
+                     (Prims.of_int (192)) (Prims.of_int (43)))))
             (Obj.magic (term_list_to_string " " witnesses))
             (fun uu___1 ->
                (fun uu___1 ->
@@ -2164,28 +2052,28 @@ let rec (st_term_to_string' :
                        (FStar_Sealed.seal
                           (Obj.magic
                              (FStar_Range.mk_range "Pulse.Syntax.Printer.fst"
-                                (Prims.of_int (190)) (Prims.of_int (6))
-                                (Prims.of_int (194)) (Prims.of_int (43)))))
+                                (Prims.of_int (188)) (Prims.of_int (6))
+                                (Prims.of_int (192)) (Prims.of_int (43)))))
                        (FStar_Sealed.seal
                           (Obj.magic
                              (FStar_Range.mk_range "Pulse.Syntax.Printer.fst"
-                                (Prims.of_int (190)) (Prims.of_int (6))
-                                (Prims.of_int (194)) (Prims.of_int (43)))))
+                                (Prims.of_int (188)) (Prims.of_int (6))
+                                (Prims.of_int (192)) (Prims.of_int (43)))))
                        (Obj.magic
                           (FStar_Tactics_Effect.tac_bind
                              (FStar_Sealed.seal
                                 (Obj.magic
                                    (FStar_Range.mk_range
                                       "Pulse.Syntax.Printer.fst"
-                                      (Prims.of_int (190)) (Prims.of_int (6))
-                                      (Prims.of_int (194))
+                                      (Prims.of_int (188)) (Prims.of_int (6))
+                                      (Prims.of_int (192))
                                       (Prims.of_int (43)))))
                              (FStar_Sealed.seal
                                 (Obj.magic
                                    (FStar_Range.mk_range
                                       "Pulse.Syntax.Printer.fst"
-                                      (Prims.of_int (190)) (Prims.of_int (6))
-                                      (Prims.of_int (194))
+                                      (Prims.of_int (188)) (Prims.of_int (6))
+                                      (Prims.of_int (192))
                                       (Prims.of_int (43)))))
                              (Obj.magic
                                 (FStar_Tactics_Effect.tac_bind
@@ -2193,9 +2081,9 @@ let rec (st_term_to_string' :
                                       (Obj.magic
                                          (FStar_Range.mk_range
                                             "Pulse.Syntax.Printer.fst"
-                                            (Prims.of_int (192))
+                                            (Prims.of_int (190))
                                             (Prims.of_int (8))
-                                            (Prims.of_int (192))
+                                            (Prims.of_int (190))
                                             (Prims.of_int (42)))))
                                    (FStar_Sealed.seal
                                       (Obj.magic
@@ -2239,13 +2127,13 @@ let rec (st_term_to_string' :
             (FStar_Sealed.seal
                (Obj.magic
                   (FStar_Range.mk_range "Pulse.Syntax.Printer.fst"
-                     (Prims.of_int (201)) (Prims.of_int (8))
-                     (Prims.of_int (201)) (Prims.of_int (43)))))
+                     (Prims.of_int (199)) (Prims.of_int (8))
+                     (Prims.of_int (199)) (Prims.of_int (43)))))
             (FStar_Sealed.seal
                (Obj.magic
                   (FStar_Range.mk_range "Pulse.Syntax.Printer.fst"
-                     (Prims.of_int (197)) (Prims.of_int (6))
-                     (Prims.of_int (201)) (Prims.of_int (43)))))
+                     (Prims.of_int (195)) (Prims.of_int (6))
+                     (Prims.of_int (199)) (Prims.of_int (43)))))
             (Obj.magic (term_list_to_string " " witnesses))
             (fun uu___1 ->
                (fun uu___1 ->
@@ -2254,28 +2142,28 @@ let rec (st_term_to_string' :
                        (FStar_Sealed.seal
                           (Obj.magic
                              (FStar_Range.mk_range "Pulse.Syntax.Printer.fst"
-                                (Prims.of_int (197)) (Prims.of_int (6))
-                                (Prims.of_int (201)) (Prims.of_int (43)))))
+                                (Prims.of_int (195)) (Prims.of_int (6))
+                                (Prims.of_int (199)) (Prims.of_int (43)))))
                        (FStar_Sealed.seal
                           (Obj.magic
                              (FStar_Range.mk_range "Pulse.Syntax.Printer.fst"
-                                (Prims.of_int (197)) (Prims.of_int (6))
-                                (Prims.of_int (201)) (Prims.of_int (43)))))
+                                (Prims.of_int (195)) (Prims.of_int (6))
+                                (Prims.of_int (199)) (Prims.of_int (43)))))
                        (Obj.magic
                           (FStar_Tactics_Effect.tac_bind
                              (FStar_Sealed.seal
                                 (Obj.magic
                                    (FStar_Range.mk_range
                                       "Pulse.Syntax.Printer.fst"
-                                      (Prims.of_int (197)) (Prims.of_int (6))
-                                      (Prims.of_int (201))
+                                      (Prims.of_int (195)) (Prims.of_int (6))
+                                      (Prims.of_int (199))
                                       (Prims.of_int (43)))))
                              (FStar_Sealed.seal
                                 (Obj.magic
                                    (FStar_Range.mk_range
                                       "Pulse.Syntax.Printer.fst"
-                                      (Prims.of_int (197)) (Prims.of_int (6))
-                                      (Prims.of_int (201))
+                                      (Prims.of_int (195)) (Prims.of_int (6))
+                                      (Prims.of_int (199))
                                       (Prims.of_int (43)))))
                              (Obj.magic
                                 (FStar_Tactics_Effect.tac_bind
@@ -2283,9 +2171,9 @@ let rec (st_term_to_string' :
                                       (Obj.magic
                                          (FStar_Range.mk_range
                                             "Pulse.Syntax.Printer.fst"
-                                            (Prims.of_int (199))
+                                            (Prims.of_int (197))
                                             (Prims.of_int (8))
-                                            (Prims.of_int (199))
+                                            (Prims.of_int (197))
                                             (Prims.of_int (42)))))
                                    (FStar_Sealed.seal
                                       (Obj.magic
@@ -2330,25 +2218,25 @@ let rec (st_term_to_string' :
             (FStar_Sealed.seal
                (Obj.magic
                   (FStar_Range.mk_range "Pulse.Syntax.Printer.fst"
-                     (Prims.of_int (204)) (Prims.of_int (6))
-                     (Prims.of_int (211)) (Prims.of_int (13)))))
+                     (Prims.of_int (202)) (Prims.of_int (6))
+                     (Prims.of_int (209)) (Prims.of_int (13)))))
             (FStar_Sealed.seal
                (Obj.magic
                   (FStar_Range.mk_range "Pulse.Syntax.Printer.fst"
-                     (Prims.of_int (204)) (Prims.of_int (6))
-                     (Prims.of_int (211)) (Prims.of_int (13)))))
+                     (Prims.of_int (202)) (Prims.of_int (6))
+                     (Prims.of_int (209)) (Prims.of_int (13)))))
             (Obj.magic
                (FStar_Tactics_Effect.tac_bind
                   (FStar_Sealed.seal
                      (Obj.magic
                         (FStar_Range.mk_range "Pulse.Syntax.Printer.fst"
-                           (Prims.of_int (210)) (Prims.of_int (8))
-                           (Prims.of_int (210)) (Prims.of_int (48)))))
+                           (Prims.of_int (208)) (Prims.of_int (8))
+                           (Prims.of_int (208)) (Prims.of_int (48)))))
                   (FStar_Sealed.seal
                      (Obj.magic
                         (FStar_Range.mk_range "Pulse.Syntax.Printer.fst"
-                           (Prims.of_int (204)) (Prims.of_int (6))
-                           (Prims.of_int (211)) (Prims.of_int (13)))))
+                           (Prims.of_int (202)) (Prims.of_int (6))
+                           (Prims.of_int (209)) (Prims.of_int (13)))))
                   (Obj.magic (st_term_to_string' (indent level) body))
                   (fun uu___1 ->
                      (fun uu___1 ->
@@ -2358,15 +2246,15 @@ let rec (st_term_to_string' :
                                 (Obj.magic
                                    (FStar_Range.mk_range
                                       "Pulse.Syntax.Printer.fst"
-                                      (Prims.of_int (204)) (Prims.of_int (6))
-                                      (Prims.of_int (211))
+                                      (Prims.of_int (202)) (Prims.of_int (6))
+                                      (Prims.of_int (209))
                                       (Prims.of_int (13)))))
                              (FStar_Sealed.seal
                                 (Obj.magic
                                    (FStar_Range.mk_range
                                       "Pulse.Syntax.Printer.fst"
-                                      (Prims.of_int (204)) (Prims.of_int (6))
-                                      (Prims.of_int (211))
+                                      (Prims.of_int (202)) (Prims.of_int (6))
+                                      (Prims.of_int (209))
                                       (Prims.of_int (13)))))
                              (Obj.magic
                                 (FStar_Tactics_Effect.tac_bind
@@ -2374,17 +2262,17 @@ let rec (st_term_to_string' :
                                       (Obj.magic
                                          (FStar_Range.mk_range
                                             "Pulse.Syntax.Printer.fst"
-                                            (Prims.of_int (204))
+                                            (Prims.of_int (202))
                                             (Prims.of_int (6))
-                                            (Prims.of_int (211))
+                                            (Prims.of_int (209))
                                             (Prims.of_int (13)))))
                                    (FStar_Sealed.seal
                                       (Obj.magic
                                          (FStar_Range.mk_range
                                             "Pulse.Syntax.Printer.fst"
-                                            (Prims.of_int (204))
+                                            (Prims.of_int (202))
                                             (Prims.of_int (6))
-                                            (Prims.of_int (211))
+                                            (Prims.of_int (209))
                                             (Prims.of_int (13)))))
                                    (Obj.magic
                                       (FStar_Tactics_Effect.tac_bind
@@ -2392,17 +2280,17 @@ let rec (st_term_to_string' :
                                             (Obj.magic
                                                (FStar_Range.mk_range
                                                   "Pulse.Syntax.Printer.fst"
-                                                  (Prims.of_int (204))
+                                                  (Prims.of_int (202))
                                                   (Prims.of_int (6))
-                                                  (Prims.of_int (211))
+                                                  (Prims.of_int (209))
                                                   (Prims.of_int (13)))))
                                          (FStar_Sealed.seal
                                             (Obj.magic
                                                (FStar_Range.mk_range
                                                   "Pulse.Syntax.Printer.fst"
-                                                  (Prims.of_int (204))
+                                                  (Prims.of_int (202))
                                                   (Prims.of_int (6))
-                                                  (Prims.of_int (211))
+                                                  (Prims.of_int (209))
                                                   (Prims.of_int (13)))))
                                          (Obj.magic
                                             (FStar_Tactics_Effect.tac_bind
@@ -2410,17 +2298,17 @@ let rec (st_term_to_string' :
                                                   (Obj.magic
                                                      (FStar_Range.mk_range
                                                         "Pulse.Syntax.Printer.fst"
-                                                        (Prims.of_int (207))
+                                                        (Prims.of_int (205))
                                                         (Prims.of_int (8))
-                                                        (Prims.of_int (207))
+                                                        (Prims.of_int (205))
                                                         (Prims.of_int (34)))))
                                                (FStar_Sealed.seal
                                                   (Obj.magic
                                                      (FStar_Range.mk_range
                                                         "Pulse.Syntax.Printer.fst"
-                                                        (Prims.of_int (204))
+                                                        (Prims.of_int (202))
                                                         (Prims.of_int (6))
-                                                        (Prims.of_int (211))
+                                                        (Prims.of_int (209))
                                                         (Prims.of_int (13)))))
                                                (Obj.magic
                                                   (term_to_string invariant))
@@ -2432,17 +2320,17 @@ let rec (st_term_to_string' :
                                                              (Obj.magic
                                                                 (FStar_Range.mk_range
                                                                    "Pulse.Syntax.Printer.fst"
-                                                                   (Prims.of_int (204))
+                                                                   (Prims.of_int (202))
                                                                    (Prims.of_int (6))
-                                                                   (Prims.of_int (211))
+                                                                   (Prims.of_int (209))
                                                                    (Prims.of_int (13)))))
                                                           (FStar_Sealed.seal
                                                              (Obj.magic
                                                                 (FStar_Range.mk_range
                                                                    "Pulse.Syntax.Printer.fst"
-                                                                   (Prims.of_int (204))
+                                                                   (Prims.of_int (202))
                                                                    (Prims.of_int (6))
-                                                                   (Prims.of_int (211))
+                                                                   (Prims.of_int (209))
                                                                    (Prims.of_int (13)))))
                                                           (Obj.magic
                                                              (FStar_Tactics_Effect.tac_bind
@@ -2450,17 +2338,17 @@ let rec (st_term_to_string' :
                                                                    (Obj.magic
                                                                     (FStar_Range.mk_range
                                                                     "Pulse.Syntax.Printer.fst"
-                                                                    (Prims.of_int (204))
+                                                                    (Prims.of_int (202))
                                                                     (Prims.of_int (6))
-                                                                    (Prims.of_int (211))
+                                                                    (Prims.of_int (209))
                                                                     (Prims.of_int (13)))))
                                                                 (FStar_Sealed.seal
                                                                    (Obj.magic
                                                                     (FStar_Range.mk_range
                                                                     "Pulse.Syntax.Printer.fst"
-                                                                    (Prims.of_int (204))
+                                                                    (Prims.of_int (202))
                                                                     (Prims.of_int (6))
-                                                                    (Prims.of_int (211))
+                                                                    (Prims.of_int (209))
                                                                     (Prims.of_int (13)))))
                                                                 (Obj.magic
                                                                    (FStar_Tactics_Effect.tac_bind
@@ -2468,9 +2356,9 @@ let rec (st_term_to_string' :
                                                                     (Obj.magic
                                                                     (FStar_Range.mk_range
                                                                     "Pulse.Syntax.Printer.fst"
-                                                                    (Prims.of_int (205))
+                                                                    (Prims.of_int (203))
                                                                     (Prims.of_int (8))
-                                                                    (Prims.of_int (205))
+                                                                    (Prims.of_int (203))
                                                                     (Prims.of_int (44)))))
                                                                     (FStar_Sealed.seal
                                                                     (Obj.magic
@@ -2544,22 +2432,22 @@ let rec (st_term_to_string' :
             (fun uu___1 ->
                FStar_Tactics_Effect.lift_div_tac (fun uu___2 -> uu___1 level))
       | Pulse_Syntax_Base.Tm_Par
-          { Pulse_Syntax_Base.pre11 = pre1; Pulse_Syntax_Base.body11 = body1;
+          { Pulse_Syntax_Base.pre1 = pre1; Pulse_Syntax_Base.body11 = body1;
             Pulse_Syntax_Base.post11 = post1; Pulse_Syntax_Base.pre2 = pre2;
             Pulse_Syntax_Base.body21 = body2;
-            Pulse_Syntax_Base.post21 = post2;_}
+            Pulse_Syntax_Base.post2 = post2;_}
           ->
           FStar_Tactics_Effect.tac_bind
             (FStar_Sealed.seal
                (Obj.magic
                   (FStar_Range.mk_range "Pulse.Syntax.Printer.fst"
-                     (Prims.of_int (220)) (Prims.of_int (8))
-                     (Prims.of_int (220)) (Prims.of_int (30)))))
+                     (Prims.of_int (218)) (Prims.of_int (8))
+                     (Prims.of_int (218)) (Prims.of_int (30)))))
             (FStar_Sealed.seal
                (Obj.magic
                   (FStar_Range.mk_range "Pulse.Syntax.Printer.fst"
-                     (Prims.of_int (214)) (Prims.of_int (6))
-                     (Prims.of_int (220)) (Prims.of_int (30)))))
+                     (Prims.of_int (212)) (Prims.of_int (6))
+                     (Prims.of_int (218)) (Prims.of_int (30)))))
             (Obj.magic (term_to_string post2))
             (fun uu___ ->
                (fun uu___ ->
@@ -2568,28 +2456,28 @@ let rec (st_term_to_string' :
                        (FStar_Sealed.seal
                           (Obj.magic
                              (FStar_Range.mk_range "Pulse.Syntax.Printer.fst"
-                                (Prims.of_int (214)) (Prims.of_int (6))
-                                (Prims.of_int (220)) (Prims.of_int (30)))))
+                                (Prims.of_int (212)) (Prims.of_int (6))
+                                (Prims.of_int (218)) (Prims.of_int (30)))))
                        (FStar_Sealed.seal
                           (Obj.magic
                              (FStar_Range.mk_range "Pulse.Syntax.Printer.fst"
-                                (Prims.of_int (214)) (Prims.of_int (6))
-                                (Prims.of_int (220)) (Prims.of_int (30)))))
+                                (Prims.of_int (212)) (Prims.of_int (6))
+                                (Prims.of_int (218)) (Prims.of_int (30)))))
                        (Obj.magic
                           (FStar_Tactics_Effect.tac_bind
                              (FStar_Sealed.seal
                                 (Obj.magic
                                    (FStar_Range.mk_range
                                       "Pulse.Syntax.Printer.fst"
-                                      (Prims.of_int (219)) (Prims.of_int (8))
-                                      (Prims.of_int (219))
+                                      (Prims.of_int (217)) (Prims.of_int (8))
+                                      (Prims.of_int (217))
                                       (Prims.of_int (40)))))
                              (FStar_Sealed.seal
                                 (Obj.magic
                                    (FStar_Range.mk_range
                                       "Pulse.Syntax.Printer.fst"
-                                      (Prims.of_int (214)) (Prims.of_int (6))
-                                      (Prims.of_int (220))
+                                      (Prims.of_int (212)) (Prims.of_int (6))
+                                      (Prims.of_int (218))
                                       (Prims.of_int (30)))))
                              (Obj.magic (st_term_to_string' level body2))
                              (fun uu___1 ->
@@ -2600,17 +2488,17 @@ let rec (st_term_to_string' :
                                            (Obj.magic
                                               (FStar_Range.mk_range
                                                  "Pulse.Syntax.Printer.fst"
-                                                 (Prims.of_int (214))
+                                                 (Prims.of_int (212))
                                                  (Prims.of_int (6))
-                                                 (Prims.of_int (220))
+                                                 (Prims.of_int (218))
                                                  (Prims.of_int (30)))))
                                         (FStar_Sealed.seal
                                            (Obj.magic
                                               (FStar_Range.mk_range
                                                  "Pulse.Syntax.Printer.fst"
-                                                 (Prims.of_int (214))
+                                                 (Prims.of_int (212))
                                                  (Prims.of_int (6))
-                                                 (Prims.of_int (220))
+                                                 (Prims.of_int (218))
                                                  (Prims.of_int (30)))))
                                         (Obj.magic
                                            (FStar_Tactics_Effect.tac_bind
@@ -2618,17 +2506,17 @@ let rec (st_term_to_string' :
                                                  (Obj.magic
                                                     (FStar_Range.mk_range
                                                        "Pulse.Syntax.Printer.fst"
-                                                       (Prims.of_int (218))
+                                                       (Prims.of_int (216))
                                                        (Prims.of_int (8))
-                                                       (Prims.of_int (218))
+                                                       (Prims.of_int (216))
                                                        (Prims.of_int (29)))))
                                               (FStar_Sealed.seal
                                                  (Obj.magic
                                                     (FStar_Range.mk_range
                                                        "Pulse.Syntax.Printer.fst"
-                                                       (Prims.of_int (214))
+                                                       (Prims.of_int (212))
                                                        (Prims.of_int (6))
-                                                       (Prims.of_int (220))
+                                                       (Prims.of_int (218))
                                                        (Prims.of_int (30)))))
                                               (Obj.magic
                                                  (term_to_string pre2))
@@ -2640,17 +2528,17 @@ let rec (st_term_to_string' :
                                                             (Obj.magic
                                                                (FStar_Range.mk_range
                                                                   "Pulse.Syntax.Printer.fst"
-                                                                  (Prims.of_int (214))
+                                                                  (Prims.of_int (212))
                                                                   (Prims.of_int (6))
-                                                                  (Prims.of_int (220))
+                                                                  (Prims.of_int (218))
                                                                   (Prims.of_int (30)))))
                                                          (FStar_Sealed.seal
                                                             (Obj.magic
                                                                (FStar_Range.mk_range
                                                                   "Pulse.Syntax.Printer.fst"
-                                                                  (Prims.of_int (214))
+                                                                  (Prims.of_int (212))
                                                                   (Prims.of_int (6))
-                                                                  (Prims.of_int (220))
+                                                                  (Prims.of_int (218))
                                                                   (Prims.of_int (30)))))
                                                          (Obj.magic
                                                             (FStar_Tactics_Effect.tac_bind
@@ -2658,17 +2546,17 @@ let rec (st_term_to_string' :
                                                                   (Obj.magic
                                                                     (FStar_Range.mk_range
                                                                     "Pulse.Syntax.Printer.fst"
-                                                                    (Prims.of_int (217))
+                                                                    (Prims.of_int (215))
                                                                     (Prims.of_int (8))
-                                                                    (Prims.of_int (217))
+                                                                    (Prims.of_int (215))
                                                                     (Prims.of_int (30)))))
                                                                (FStar_Sealed.seal
                                                                   (Obj.magic
                                                                     (FStar_Range.mk_range
                                                                     "Pulse.Syntax.Printer.fst"
-                                                                    (Prims.of_int (214))
+                                                                    (Prims.of_int (212))
                                                                     (Prims.of_int (6))
-                                                                    (Prims.of_int (220))
+                                                                    (Prims.of_int (218))
                                                                     (Prims.of_int (30)))))
                                                                (Obj.magic
                                                                   (term_to_string
@@ -2682,17 +2570,17 @@ let rec (st_term_to_string' :
                                                                     (Obj.magic
                                                                     (FStar_Range.mk_range
                                                                     "Pulse.Syntax.Printer.fst"
-                                                                    (Prims.of_int (214))
+                                                                    (Prims.of_int (212))
                                                                     (Prims.of_int (6))
-                                                                    (Prims.of_int (220))
+                                                                    (Prims.of_int (218))
                                                                     (Prims.of_int (30)))))
                                                                     (FStar_Sealed.seal
                                                                     (Obj.magic
                                                                     (FStar_Range.mk_range
                                                                     "Pulse.Syntax.Printer.fst"
-                                                                    (Prims.of_int (214))
+                                                                    (Prims.of_int (212))
                                                                     (Prims.of_int (6))
-                                                                    (Prims.of_int (220))
+                                                                    (Prims.of_int (218))
                                                                     (Prims.of_int (30)))))
                                                                     (Obj.magic
                                                                     (FStar_Tactics_Effect.tac_bind
@@ -2700,17 +2588,17 @@ let rec (st_term_to_string' :
                                                                     (Obj.magic
                                                                     (FStar_Range.mk_range
                                                                     "Pulse.Syntax.Printer.fst"
-                                                                    (Prims.of_int (216))
+                                                                    (Prims.of_int (214))
                                                                     (Prims.of_int (8))
-                                                                    (Prims.of_int (216))
+                                                                    (Prims.of_int (214))
                                                                     (Prims.of_int (40)))))
                                                                     (FStar_Sealed.seal
                                                                     (Obj.magic
                                                                     (FStar_Range.mk_range
                                                                     "Pulse.Syntax.Printer.fst"
-                                                                    (Prims.of_int (214))
+                                                                    (Prims.of_int (212))
                                                                     (Prims.of_int (6))
-                                                                    (Prims.of_int (220))
+                                                                    (Prims.of_int (218))
                                                                     (Prims.of_int (30)))))
                                                                     (Obj.magic
                                                                     (st_term_to_string'
@@ -2726,17 +2614,17 @@ let rec (st_term_to_string' :
                                                                     (Obj.magic
                                                                     (FStar_Range.mk_range
                                                                     "Pulse.Syntax.Printer.fst"
-                                                                    (Prims.of_int (214))
+                                                                    (Prims.of_int (212))
                                                                     (Prims.of_int (6))
-                                                                    (Prims.of_int (220))
+                                                                    (Prims.of_int (218))
                                                                     (Prims.of_int (30)))))
                                                                     (FStar_Sealed.seal
                                                                     (Obj.magic
                                                                     (FStar_Range.mk_range
                                                                     "Pulse.Syntax.Printer.fst"
-                                                                    (Prims.of_int (214))
+                                                                    (Prims.of_int (212))
                                                                     (Prims.of_int (6))
-                                                                    (Prims.of_int (220))
+                                                                    (Prims.of_int (218))
                                                                     (Prims.of_int (30)))))
                                                                     (Obj.magic
                                                                     (FStar_Tactics_Effect.tac_bind
@@ -2744,9 +2632,9 @@ let rec (st_term_to_string' :
                                                                     (Obj.magic
                                                                     (FStar_Range.mk_range
                                                                     "Pulse.Syntax.Printer.fst"
-                                                                    (Prims.of_int (215))
+                                                                    (Prims.of_int (213))
                                                                     (Prims.of_int (8))
-                                                                    (Prims.of_int (215))
+                                                                    (Prims.of_int (213))
                                                                     (Prims.of_int (29)))))
                                                                     (FStar_Sealed.seal
                                                                     (Obj.magic
@@ -2824,13 +2712,13 @@ let rec (st_term_to_string' :
             (FStar_Sealed.seal
                (Obj.magic
                   (FStar_Range.mk_range "Pulse.Syntax.Printer.fst"
-                     (Prims.of_int (225)) (Prims.of_int (15))
-                     (Prims.of_int (225)) (Prims.of_int (34)))))
+                     (Prims.of_int (223)) (Prims.of_int (15))
+                     (Prims.of_int (223)) (Prims.of_int (34)))))
             (FStar_Sealed.seal
                (Obj.magic
                   (FStar_Range.mk_range "Pulse.Syntax.Printer.fst"
-                     (Prims.of_int (223)) (Prims.of_int (7))
-                     (Prims.of_int (225)) (Prims.of_int (34)))))
+                     (Prims.of_int (221)) (Prims.of_int (7))
+                     (Prims.of_int (223)) (Prims.of_int (34)))))
             (Obj.magic (term_to_string t2))
             (fun uu___ ->
                (fun uu___ ->
@@ -2839,21 +2727,21 @@ let rec (st_term_to_string' :
                        (FStar_Sealed.seal
                           (Obj.magic
                              (FStar_Range.mk_range "Pulse.Syntax.Printer.fst"
-                                (Prims.of_int (223)) (Prims.of_int (7))
-                                (Prims.of_int (225)) (Prims.of_int (34)))))
+                                (Prims.of_int (221)) (Prims.of_int (7))
+                                (Prims.of_int (223)) (Prims.of_int (34)))))
                        (FStar_Sealed.seal
                           (Obj.magic
                              (FStar_Range.mk_range "Pulse.Syntax.Printer.fst"
-                                (Prims.of_int (223)) (Prims.of_int (7))
-                                (Prims.of_int (225)) (Prims.of_int (34)))))
+                                (Prims.of_int (221)) (Prims.of_int (7))
+                                (Prims.of_int (223)) (Prims.of_int (34)))))
                        (Obj.magic
                           (FStar_Tactics_Effect.tac_bind
                              (FStar_Sealed.seal
                                 (Obj.magic
                                    (FStar_Range.mk_range
                                       "Pulse.Syntax.Printer.fst"
-                                      (Prims.of_int (224)) (Prims.of_int (8))
-                                      (Prims.of_int (224))
+                                      (Prims.of_int (222)) (Prims.of_int (8))
+                                      (Prims.of_int (222))
                                       (Prims.of_int (27)))))
                              (FStar_Sealed.seal
                                 (Obj.magic
@@ -2882,13 +2770,13 @@ let rec (st_term_to_string' :
             (FStar_Sealed.seal
                (Obj.magic
                   (FStar_Range.mk_range "Pulse.Syntax.Printer.fst"
-                     (Prims.of_int (231)) (Prims.of_int (8))
-                     (Prims.of_int (231)) (Prims.of_int (39)))))
+                     (Prims.of_int (229)) (Prims.of_int (8))
+                     (Prims.of_int (229)) (Prims.of_int (39)))))
             (FStar_Sealed.seal
                (Obj.magic
                   (FStar_Range.mk_range "Pulse.Syntax.Printer.fst"
-                     (Prims.of_int (228)) (Prims.of_int (6))
-                     (Prims.of_int (231)) (Prims.of_int (39)))))
+                     (Prims.of_int (226)) (Prims.of_int (6))
+                     (Prims.of_int (229)) (Prims.of_int (39)))))
             (Obj.magic (st_term_to_string' level body))
             (fun uu___1 ->
                (fun uu___1 ->
@@ -2897,28 +2785,28 @@ let rec (st_term_to_string' :
                        (FStar_Sealed.seal
                           (Obj.magic
                              (FStar_Range.mk_range "Pulse.Syntax.Printer.fst"
-                                (Prims.of_int (228)) (Prims.of_int (6))
-                                (Prims.of_int (231)) (Prims.of_int (39)))))
+                                (Prims.of_int (226)) (Prims.of_int (6))
+                                (Prims.of_int (229)) (Prims.of_int (39)))))
                        (FStar_Sealed.seal
                           (Obj.magic
                              (FStar_Range.mk_range "Pulse.Syntax.Printer.fst"
-                                (Prims.of_int (228)) (Prims.of_int (6))
-                                (Prims.of_int (231)) (Prims.of_int (39)))))
+                                (Prims.of_int (226)) (Prims.of_int (6))
+                                (Prims.of_int (229)) (Prims.of_int (39)))))
                        (Obj.magic
                           (FStar_Tactics_Effect.tac_bind
                              (FStar_Sealed.seal
                                 (Obj.magic
                                    (FStar_Range.mk_range
                                       "Pulse.Syntax.Printer.fst"
-                                      (Prims.of_int (228)) (Prims.of_int (6))
-                                      (Prims.of_int (231))
+                                      (Prims.of_int (226)) (Prims.of_int (6))
+                                      (Prims.of_int (229))
                                       (Prims.of_int (39)))))
                              (FStar_Sealed.seal
                                 (Obj.magic
                                    (FStar_Range.mk_range
                                       "Pulse.Syntax.Printer.fst"
-                                      (Prims.of_int (228)) (Prims.of_int (6))
-                                      (Prims.of_int (231))
+                                      (Prims.of_int (226)) (Prims.of_int (6))
+                                      (Prims.of_int (229))
                                       (Prims.of_int (39)))))
                              (Obj.magic
                                 (FStar_Tactics_Effect.tac_bind
@@ -2926,9 +2814,9 @@ let rec (st_term_to_string' :
                                       (Obj.magic
                                          (FStar_Range.mk_range
                                             "Pulse.Syntax.Printer.fst"
-                                            (Prims.of_int (229))
+                                            (Prims.of_int (227))
                                             (Prims.of_int (8))
-                                            (Prims.of_int (229))
+                                            (Prims.of_int (227))
                                             (Prims.of_int (36)))))
                                    (FStar_Sealed.seal
                                       (Obj.magic
@@ -2966,13 +2854,13 @@ let rec (st_term_to_string' :
             (FStar_Sealed.seal
                (Obj.magic
                   (FStar_Range.mk_range "Pulse.Syntax.Printer.fst"
-                     (Prims.of_int (241)) (Prims.of_int (8))
-                     (Prims.of_int (243)) (Prims.of_int (60)))))
+                     (Prims.of_int (239)) (Prims.of_int (8))
+                     (Prims.of_int (241)) (Prims.of_int (60)))))
             (FStar_Sealed.seal
                (Obj.magic
                   (FStar_Range.mk_range "Pulse.Syntax.Printer.fst"
-                     (Prims.of_int (234)) (Prims.of_int (6))
-                     (Prims.of_int (243)) (Prims.of_int (60)))))
+                     (Prims.of_int (232)) (Prims.of_int (6))
+                     (Prims.of_int (241)) (Prims.of_int (60)))))
             (match post with
              | FStar_Pervasives_Native.None ->
                  Obj.magic
@@ -2986,8 +2874,8 @@ let rec (st_term_to_string' :
                             (Obj.magic
                                (FStar_Range.mk_range
                                   "Pulse.Syntax.Printer.fst"
-                                  (Prims.of_int (243)) (Prims.of_int (38))
-                                  (Prims.of_int (243)) (Prims.of_int (59)))))
+                                  (Prims.of_int (241)) (Prims.of_int (38))
+                                  (Prims.of_int (241)) (Prims.of_int (59)))))
                          (FStar_Sealed.seal
                             (Obj.magic
                                (FStar_Range.mk_range "prims.fst"
@@ -3005,21 +2893,21 @@ let rec (st_term_to_string' :
                        (FStar_Sealed.seal
                           (Obj.magic
                              (FStar_Range.mk_range "Pulse.Syntax.Printer.fst"
-                                (Prims.of_int (234)) (Prims.of_int (6))
-                                (Prims.of_int (243)) (Prims.of_int (60)))))
+                                (Prims.of_int (232)) (Prims.of_int (6))
+                                (Prims.of_int (241)) (Prims.of_int (60)))))
                        (FStar_Sealed.seal
                           (Obj.magic
                              (FStar_Range.mk_range "Pulse.Syntax.Printer.fst"
-                                (Prims.of_int (234)) (Prims.of_int (6))
-                                (Prims.of_int (243)) (Prims.of_int (60)))))
+                                (Prims.of_int (232)) (Prims.of_int (6))
+                                (Prims.of_int (241)) (Prims.of_int (60)))))
                        (Obj.magic
                           (FStar_Tactics_Effect.tac_bind
                              (FStar_Sealed.seal
                                 (Obj.magic
                                    (FStar_Range.mk_range
                                       "Pulse.Syntax.Printer.fst"
-                                      (Prims.of_int (240)) (Prims.of_int (8))
-                                      (Prims.of_int (240))
+                                      (Prims.of_int (238)) (Prims.of_int (8))
+                                      (Prims.of_int (238))
                                       (Prims.of_int (28)))))
                              (FStar_Sealed.seal
                                 (Obj.magic
@@ -3060,8 +2948,8 @@ let rec (st_term_to_string' :
             (FStar_Sealed.seal
                (Obj.magic
                   (FStar_Range.mk_range "Pulse.Syntax.Printer.fst"
-                     (Prims.of_int (248)) (Prims.of_int (6))
-                     (Prims.of_int (248)) (Prims.of_int (34)))))
+                     (Prims.of_int (246)) (Prims.of_int (6))
+                     (Prims.of_int (246)) (Prims.of_int (34)))))
             (FStar_Sealed.seal
                (Obj.magic
                   (FStar_Range.mk_range "prims.fst" (Prims.of_int (590))
@@ -3083,13 +2971,13 @@ let rec (st_term_to_string' :
             (FStar_Sealed.seal
                (Obj.magic
                   (FStar_Range.mk_range "Pulse.Syntax.Printer.fst"
-                     (Prims.of_int (253)) (Prims.of_int (8))
-                     (Prims.of_int (253)) (Prims.of_int (36)))))
+                     (Prims.of_int (251)) (Prims.of_int (8))
+                     (Prims.of_int (251)) (Prims.of_int (36)))))
             (FStar_Sealed.seal
                (Obj.magic
                   (FStar_Range.mk_range "Pulse.Syntax.Printer.fst"
-                     (Prims.of_int (251)) (Prims.of_int (6))
-                     (Prims.of_int (253)) (Prims.of_int (36)))))
+                     (Prims.of_int (249)) (Prims.of_int (6))
+                     (Prims.of_int (251)) (Prims.of_int (36)))))
             (Obj.magic (st_term_to_string' level t1))
             (fun uu___1 ->
                (fun uu___1 ->
@@ -3098,21 +2986,21 @@ let rec (st_term_to_string' :
                        (FStar_Sealed.seal
                           (Obj.magic
                              (FStar_Range.mk_range "Pulse.Syntax.Printer.fst"
-                                (Prims.of_int (251)) (Prims.of_int (6))
-                                (Prims.of_int (253)) (Prims.of_int (36)))))
+                                (Prims.of_int (249)) (Prims.of_int (6))
+                                (Prims.of_int (251)) (Prims.of_int (36)))))
                        (FStar_Sealed.seal
                           (Obj.magic
                              (FStar_Range.mk_range "Pulse.Syntax.Printer.fst"
-                                (Prims.of_int (251)) (Prims.of_int (6))
-                                (Prims.of_int (253)) (Prims.of_int (36)))))
+                                (Prims.of_int (249)) (Prims.of_int (6))
+                                (Prims.of_int (251)) (Prims.of_int (36)))))
                        (Obj.magic
                           (FStar_Tactics_Effect.tac_bind
                              (FStar_Sealed.seal
                                 (Obj.magic
                                    (FStar_Range.mk_range
                                       "Pulse.Syntax.Printer.fst"
-                                      (Prims.of_int (252)) (Prims.of_int (8))
-                                      (Prims.of_int (252))
+                                      (Prims.of_int (250)) (Prims.of_int (8))
+                                      (Prims.of_int (250))
                                       (Prims.of_int (26)))))
                              (FStar_Sealed.seal
                                 (Obj.magic
@@ -3169,6 +3057,60 @@ let (tag_of_st_term : Pulse_Syntax_Base.st_term -> Prims.string) =
     | Pulse_Syntax_Base.Tm_Protect uu___ -> "Tm_Protect"
     | Pulse_Syntax_Base.Tm_ProofHintWithBinders uu___ ->
         "Tm_ProofHintWithBinders"
+let (tag_of_comp :
+  Pulse_Syntax_Base.comp ->
+    (Prims.string, unit) FStar_Tactics_Effect.tac_repr)
+  =
+  fun uu___ ->
+    (fun c ->
+       match c with
+       | Pulse_Syntax_Base.C_Tot uu___ ->
+           Obj.magic
+             (Obj.repr
+                (FStar_Tactics_Effect.lift_div_tac (fun uu___1 -> "Total")))
+       | Pulse_Syntax_Base.C_ST uu___ ->
+           Obj.magic
+             (Obj.repr
+                (FStar_Tactics_Effect.lift_div_tac (fun uu___1 -> "ST")))
+       | Pulse_Syntax_Base.C_STAtomic (i, uu___) ->
+           Obj.magic
+             (Obj.repr
+                (FStar_Tactics_Effect.tac_bind
+                   (FStar_Sealed.seal
+                      (Obj.magic
+                         (FStar_Range.mk_range "Pulse.Syntax.Printer.fst"
+                            (Prims.of_int (293)) (Prims.of_int (31))
+                            (Prims.of_int (293)) (Prims.of_int (49)))))
+                   (FStar_Sealed.seal
+                      (Obj.magic
+                         (FStar_Range.mk_range "prims.fst"
+                            (Prims.of_int (590)) (Prims.of_int (19))
+                            (Prims.of_int (590)) (Prims.of_int (31)))))
+                   (Obj.magic (term_to_string i))
+                   (fun uu___1 ->
+                      FStar_Tactics_Effect.lift_div_tac
+                        (fun uu___2 ->
+                           Prims.strcat "Atomic " (Prims.strcat uu___1 "")))))
+       | Pulse_Syntax_Base.C_STGhost (i, uu___) ->
+           Obj.magic
+             (Obj.repr
+                (FStar_Tactics_Effect.tac_bind
+                   (FStar_Sealed.seal
+                      (Obj.magic
+                         (FStar_Range.mk_range "Pulse.Syntax.Printer.fst"
+                            (Prims.of_int (295)) (Prims.of_int (30))
+                            (Prims.of_int (295)) (Prims.of_int (48)))))
+                   (FStar_Sealed.seal
+                      (Obj.magic
+                         (FStar_Range.mk_range "prims.fst"
+                            (Prims.of_int (590)) (Prims.of_int (19))
+                            (Prims.of_int (590)) (Prims.of_int (31)))))
+                   (Obj.magic (term_to_string i))
+                   (fun uu___1 ->
+                      FStar_Tactics_Effect.lift_div_tac
+                        (fun uu___2 ->
+                           Prims.strcat "Ghost " (Prims.strcat uu___1 ""))))))
+      uu___
 let rec (print_st_head : Pulse_Syntax_Base.st_term -> Prims.string) =
   fun t ->
     match t.Pulse_Syntax_Base.term1 with
@@ -3198,9 +3140,8 @@ let rec (print_skel : Pulse_Syntax_Base.st_term -> Prims.string) =
     match t.Pulse_Syntax_Base.term1 with
     | Pulse_Syntax_Base.Tm_Abs
         { Pulse_Syntax_Base.b = uu___; Pulse_Syntax_Base.q = uu___1;
-          Pulse_Syntax_Base.pre1 = uu___2; Pulse_Syntax_Base.body = body;
-          Pulse_Syntax_Base.ret_ty = uu___3;
-          Pulse_Syntax_Base.post1 = uu___4;_}
+          Pulse_Syntax_Base.ascription = uu___2;
+          Pulse_Syntax_Base.body = body;_}
         -> Prims.strcat "(fun _ -> " (Prims.strcat (print_skel body) ")")
     | Pulse_Syntax_Base.Tm_Protect { Pulse_Syntax_Base.t3 = p;_} ->
         Prims.strcat "(Protect " (Prims.strcat (print_skel p) ")")
