pulse/lib/steel/pulse/Pulse.Syntax.Printer.fsti
@@ -14,6 +14,6 @@ val term_list_to_string (sep:string) (t:list term): T.Tac string
 val st_term_to_string (t:st_term) : T.Tac string
 val tag_of_term (t:term) : string
 val tag_of_st_term (t:st_term) : string
-
+val tag_of_comp (c:comp): T.Tac string
 val print_st_head (t:st_term) : string
 val print_skel (t:st_term) : string
