pulse/share/steel/examples/pulse/bug-reports/RecordWithRefs.fst
@@ -24,6 +24,20 @@ let u8_pair_pred (p:u8_pair) (v:u8_pair_repr) : vprop =
     R.pts_to p.a full_perm (fst v) `star`
     R.pts_to p.b full_perm (snd v)
 
+
+```pulse
+ghost
+fn fold_u8_pair_pred (x:u8_pair) (#u #v:erased U8.t)
+  requires
+    R.pts_to x.a full_perm u `star`
+    R.pts_to x.b full_perm v
+  ensures
+    u8_pair_pred x (reveal u, reveal v)
+{
+   fold (u8_pair_pred x (reveal u, reveal v))
+}
+```
+
 // [@@expect_failure]
 // ```pulse
 // fn swap_pair (p: u8_pair) (#v: erased u8_pair_repr)
@@ -105,5 +119,26 @@ fn swap_pair_alt2 (p: u8_pair) (#v: erased u8_pair_repr)
     with _v1 _v2.
     fold [fst; snd] u8_pair_pred p (_v1, _v2);
     ()
+}
+```
+
+
+
+```pulse
+fn swap_pair_alt3 (p: u8_pair) (#v: erased u8_pair_repr)
+  requires 
+    u8_pair_pred p v
+  ensures
+    u8_pair_pred p (snd v, fst v)
+{
+    with _p _v.
+    unfold (u8_pair_pred _p _v);
+    
+    let x = !p.a;
+    let y = !p.b;
+    (write p.a y);
+    (write p.b x);
+    
+    fold_u8_pair_pred p
 }
 ```
